@prefix : <http://WSP.org/ontology/cro#> .
@prefix cro: <http://WSP.org/ontology/cro#> .
@prefix ns1: <http://www.w3.org/2002/07/owl#> .
@prefix owl: <http://www.w3.org/2002/07/owl#> .
@prefix rdf: <http://www.w3.org/1999/02/22-rdf-syntax-ns#> .
@prefix xml: <http://www.w3.org/XML/1998/namespace> .
@prefix xsd: <http://www.w3.org/2001/XMLSchema#> .
@prefix rdfs: <http://www.w3.org/2000/01/rdf-schema#> .
@base <http://WSP.org/ontology/cro#> .

<http://WSP.org/ontology/cro> rdf:type owl:Ontology ;
                               owl:versionIRI <http://WSP.org/ontology/cro-1.16> .

#################################################################
#    Object Properties
#################################################################

###  http://WSP.org/ontology/cro#UpgradeThroughProject
cro:UpgradeThroughProject rdf:type owl:ObjectProperty ;
                          rdfs:comment "Specifies a specific class was upgraded or is planned to be upgraded by the effors of a project" .


###  http://WSP.org/ontology/cro#connectsFrom
cro:connectsFrom rdf:type owl:ObjectProperty ;
                 rdfs:comment "Indicates the source from which a transmission line starts, typically a power station." .


###  http://WSP.org/ontology/cro#connectsTailingsCells
cro:connectsTailingsCells rdf:type owl:ObjectProperty .


###  http://WSP.org/ontology/cro#connectsTo
cro:connectsTo rdf:type owl:ObjectProperty ;
               rdfs:comment "Indicates the destination to which a transmission line connects, typically a transformer." .


###  http://WSP.org/ontology/cro#containedIn
cro:containedIn rdf:type owl:ObjectProperty .


###  http://WSP.org/ontology/cro#definesRecommendations
cro:definesRecommendations rdf:type owl:ObjectProperty .


###  http://WSP.org/ontology/cro#distributedTo
cro:distributedTo rdf:type owl:ObjectProperty ;
                  rdfs:comment "Indicates the employee or entity to whom a document, report, or data set has been distributed." .


###  http://WSP.org/ontology/cro#hasAssumptions
cro:hasAssumptions rdf:type owl:ObjectProperty ;
                   rdfs:comment "Links Critical Risk Scenarios to Assumptions and Basis" .


###  http://WSP.org/ontology/cro#hasAuditsAndReviews
cro:hasAuditsAndReviews rdf:type owl:ObjectProperty ;
                        rdfs:comment "Specifies the audits and reviews help for the Critical Risk Assesment Report" .


###  http://WSP.org/ontology/cro#hasCatastrophicRiskScenariosWithLowProbability
cro:hasCatastrophicRiskScenariosWithLowProbability rdf:type owl:ObjectProperty ;
                                                   rdfs:comment "Links Critical Risk Scenario Overview to Catastrophic Risk Scenarios with Low Probability Overview" .


###  http://WSP.org/ontology/cro#hasCriticalRiskScenario
cro:hasCriticalRiskScenario rdf:type owl:ObjectProperty ;
                            rdfs:comment "Links Critical Risk Scenarios Overview with the actual critical risk scenarios and their descriptions." .


###  http://WSP.org/ontology/cro#hasCriticalRiskScenarioOverview
cro:hasCriticalRiskScenarioOverview rdf:type owl:ObjectProperty .


###  http://WSP.org/ontology/cro#hasDependencies
cro:hasDependencies rdf:type owl:ObjectProperty ;
                    rdfs:comment "Links Critical Risk Scenarios to Dependencies" .


###  http://WSP.org/ontology/cro#hasDieselGenerator
cro:hasDieselGenerator rdf:type owl:ObjectProperty ;
                       rdfs:comment "Indicates that a power station includes a diesel generator." .


###  http://WSP.org/ontology/cro#hasDistributionSystem
cro:hasDistributionSystem rdf:type owl:ObjectProperty ;
                          rdfs:comment "Indicates that a power network includes a distribution system." .


###  http://WSP.org/ontology/cro#hasDivision
cro:hasDivision rdf:type owl:ObjectProperty ;
                rdfs:comment "Connects a company to its divisions, each of which is responsible for a specific aspect of the company's operations." .


###  http://WSP.org/ontology/cro#hasEmbankment
cro:hasEmbankment rdf:type owl:ObjectProperty .


###  http://WSP.org/ontology/cro#hasEmployee
cro:hasEmployee rdf:type owl:ObjectProperty ;
                rdfs:comment "Links a company to the employees who work within it, as well as an employee to anmy work they have done" .


###  http://WSP.org/ontology/cro#hasEquipment
cro:hasEquipment rdf:type owl:ObjectProperty ;
                 rdfs:comment "Links a facility, operation, or process to the equipment used within it, wether its machinery, vessel, etc." .


###  http://WSP.org/ontology/cro#hasFacility
cro:hasFacility rdf:type owl:ObjectProperty ;
                rdfs:comment "Associates an operation with the facilities it encompasses, where various activities and processes are carried out." .


###  http://WSP.org/ontology/cro#hasIdentifiedCriticalRiskScenarios
cro:hasIdentifiedCriticalRiskScenarios rdf:type owl:ObjectProperty .


###  http://WSP.org/ontology/cro#hasIdentifiedRecommendations
cro:hasIdentifiedRecommendations rdf:type owl:ObjectProperty .


###  http://WSP.org/ontology/cro#hasInloading
cro:hasInloading rdf:type owl:ObjectProperty ;
                 rdfs:comment "Connects a terminal to the inloading operations that involve receiving goods or materials." .


###  http://WSP.org/ontology/cro#hasMarineOperation
cro:hasMarineOperation rdf:type owl:ObjectProperty ;
                       rdfs:comment "Denotes the marine-related operations, such as berthing, inloading, and outloading, associated with a port." .


###  http://WSP.org/ontology/cro#hasNATHANData
cro:hasNATHANData rdf:type owl:ObjectProperty ;
                  rdfs:comment "Connects a Critical Risk Assessment (CRA) to the relevant NATHAN Data, which includes risk factors such as natural disasters." .


###  http://WSP.org/ontology/cro#hasOutloading
cro:hasOutloading rdf:type owl:ObjectProperty ;
                  rdfs:comment "Links a terminal to the outloading operations that involve dispatching goods or materials." .


###  http://WSP.org/ontology/cro#hasPowerStation
cro:hasPowerStation rdf:type owl:ObjectProperty ;
                    rdfs:comment "Indicates that a power network includes a power station." .


###  http://WSP.org/ontology/cro#hasProcess
cro:hasProcess rdf:type owl:ObjectProperty ;
               rdfs:comment "Associates a facility or operation with specific processes or workflows that take place within it." .


###  http://WSP.org/ontology/cro#hasProcessControl
cro:hasProcessControl rdf:type owl:ObjectProperty .


###  http://WSP.org/ontology/cro#hasProject
cro:hasProject rdf:type owl:ObjectProperty ;
               rdfs:comment "Specifies a class has a project related to it" .


###  http://WSP.org/ontology/cro#hasRecommendation
cro:hasRecommendation rdf:type owl:ObjectProperty ;
                      rdfs:comment "Associates a critical risk scenario with its recommended actions." ,
                                   "Links Recommendations to Critical Risk Scenarios" .


###  http://WSP.org/ontology/cro#hasReferenceDocuments
cro:hasReferenceDocuments rdf:type owl:ObjectProperty ;
                          rdfs:comment "Links Survey and Report Details to Reference Documents" .


###  http://WSP.org/ontology/cro#hasRejectedRecommendations
cro:hasRejectedRecommendations rdf:type owl:ObjectProperty ;
                               rdfs:comment "Links Recommendation Overview to Rejected Recommendations Since Last Visit" .


###  http://WSP.org/ontology/cro#hasRevision
cro:hasRevision rdf:type owl:ObjectProperty ;
                rdfs:comment "Indicates the revision history or specific revision details associated with a document or assessment." .


###  http://WSP.org/ontology/cro#hasRisk
cro:hasRisk rdf:type owl:ObjectProperty ;
            rdfs:domain cro:Equipment ;
            rdfs:comment "Associates an operation or asset with a critical risk scenario." .


###  http://WSP.org/ontology/cro#hasRiskAssessmentReport
cro:hasRiskAssessmentReport rdf:type owl:ObjectProperty ;
                            rdfs:comment "Associates an operation or facility with its Critical Risk Assessments (CRAs), which evaluate potential risks." .


###  http://WSP.org/ontology/cro#hasRiskManagementSubElement
cro:hasRiskManagementSubElement rdf:type owl:ObjectProperty .


###  http://WSP.org/ontology/cro#hasRiskManagementSystem
cro:hasRiskManagementSystem rdf:type owl:ObjectProperty .


###  http://WSP.org/ontology/cro#hasSignificantChanges
cro:hasSignificantChanges rdf:type owl:ObjectProperty ;
                          rdfs:comment "Specifies that the Critical Risk Assesment Report has a significant change from the previous report." .


###  http://WSP.org/ontology/cro#hasSignificantIncidents
cro:hasSignificantIncidents rdf:type owl:ObjectProperty ;
                            rdfs:comment "Specifies that the Critical Risk Assesment Report had a significant incident since the last report." .


###  http://WSP.org/ontology/cro#hasSpillway
cro:hasSpillway rdf:type owl:ObjectProperty .


###  http://WSP.org/ontology/cro#hasSubFacility
cro:hasSubFacility rdf:type owl:ObjectProperty ;
                   rdfs:comment "Links a main facility to its associated sub-facilities, which may focus on specific operational activities." .


###  http://WSP.org/ontology/cro#hasSubstation
cro:hasSubstation rdf:type owl:ObjectProperty ;
                  rdfs:comment "Indicates that a distribution system includes a substation." .


###  http://WSP.org/ontology/cro#hasSurveyAndReportDetails
cro:hasSurveyAndReportDetails rdf:type owl:ObjectProperty .


###  http://WSP.org/ontology/cro#hasTSF
cro:hasTSF rdf:type owl:ObjectProperty .


###  http://WSP.org/ontology/cro#hasTailingsCell
cro:hasTailingsCell rdf:type owl:ObjectProperty .


###  http://WSP.org/ontology/cro#hasTerminal
cro:hasTerminal rdf:type owl:ObjectProperty ;
                rdfs:subPropertyOf cro:hasFacility ;
                rdfs:comment "Connects a port to its associated terminal(s), where loading and unloading activities occur." .


###  http://WSP.org/ontology/cro#hasTransformer
cro:hasTransformer rdf:type owl:ObjectProperty ;
                   rdfs:comment "Indicates that a transformer is located at a specific substation" .


###  http://WSP.org/ontology/cro#hasTransmissionLine
cro:hasTransmissionLine rdf:type owl:ObjectProperty ;
                        rdfs:comment "Indicates that a distribution system includes a transmission line." .


###  http://WSP.org/ontology/cro#hasTurbine
cro:hasTurbine rdf:type owl:ObjectProperty ;
               rdfs:comment "Indicates that a power station includes a turbine." .


###  http://WSP.org/ontology/cro#impactsAssetGroup
cro:impactsAssetGroup rdf:type owl:ObjectProperty ;
                      rdfs:comment "Links a Critical Risk Scenario to an Asset Group such as Port Facilities, Power Distribution and Material Handling." .


###  http://WSP.org/ontology/cro#impactsOperation
cro:impactsOperation rdf:type owl:ObjectProperty .


###  http://WSP.org/ontology/cro#improvedCriticalRiskScenario
cro:improvedCriticalRiskScenario rdf:type owl:ObjectProperty .


###  http://WSP.org/ontology/cro#improvesOperation
cro:improvesOperation rdf:type owl:ObjectProperty .


###  http://WSP.org/ontology/cro#isPartOf
cro:isPartOf rdf:type owl:ObjectProperty .


###  http://WSP.org/ontology/cro#issuedBy
cro:issuedBy rdf:type owl:ObjectProperty ;
             rdfs:comment "Specifies the employee or entity that issued a document, report, or directive." .


###  http://WSP.org/ontology/cro#operatedBy
cro:operatedBy rdf:type owl:ObjectProperty ;
               rdfs:comment "Denotes the division or entity responsible for the day-to-day operations of a facility, process, or piece of equipment." .


###  http://WSP.org/ontology/cro#ownedBy
cro:ownedBy rdf:type owl:ObjectProperty ;
            rdfs:comment "Identifies the company or entity that owns a facility, equipment, or operation." .


###  http://WSP.org/ontology/cro#preparedBy
cro:preparedBy rdf:type owl:ObjectProperty ;
               rdfs:comment "Specifies the employee responsible for preparing a specific document, report, or assessment." .


###  http://WSP.org/ontology/cro#producesTailings
cro:producesTailings rdf:type owl:ObjectProperty .


###  http://WSP.org/ontology/cro#providesOreForProcessing
cro:providesOreForProcessing rdf:type owl:ObjectProperty .


###  http://WSP.org/ontology/cro#recommendationImprovesEquipment
cro:recommendationImprovesEquipment rdf:type owl:ObjectProperty .


###  http://WSP.org/ontology/cro#recommendationImprovesFacility
cro:recommendationImprovesFacility rdf:type owl:ObjectProperty .


###  http://WSP.org/ontology/cro#responsibleFor
cro:responsibleFor rdf:type owl:ObjectProperty .


###  http://WSP.org/ontology/cro#riskImpactsEquipment
cro:riskImpactsEquipment rdf:type owl:ObjectProperty .


###  http://WSP.org/ontology/cro#riskImpactsFacility
cro:riskImpactsFacility rdf:type owl:ObjectProperty .


###  http://WSP.org/ontology/cro#riskManagementSystemImproved
cro:riskManagementSystemImproved rdf:type owl:ObjectProperty .


###  http://WSP.org/ontology/cro#suppliesPowerTo
cro:suppliesPowerTo rdf:type owl:ObjectProperty ;
                    rdfs:comment "Indicates the entity or facility that receives electrical power from a power network or station" .


###  http://WSP.org/ontology/cro#transformerLocatedAtSubstation
cro:transformerLocatedAtSubstation rdf:type owl:ObjectProperty ;
                                   rdfs:comment "Specifies the class is located at a specific place or location" .


###  http://WSP.org/ontology/cro/hasMFLRiskAssessmentReports
<http://WSP.org/ontology/cro/hasMFLRiskAssessmentReports> rdf:type owl:ObjectProperty .


###  http://WSP.org/ontology/cro/hasNLERiskAssessmentReports
<http://WSP.org/ontology/cro/hasNLERiskAssessmentReports> rdf:type owl:ObjectProperty .


#################################################################
#    Data properties
#################################################################

###  http://WSP.org/ontology/cro#BISummary
cro:BISummary rdf:type owl:DatatypeProperty .


###  http://WSP.org/ontology/cro#InstalledInYear
cro:InstalledInYear rdf:type owl:DatatypeProperty ;
                    rdfs:comment "The year when the Process Control Automation System was installed and began operation, marking the start of its service life." .


###  http://WSP.org/ontology/cro#PCASDescription
cro:PCASDescription rdf:type owl:DatatypeProperty ;
                    rdfs:subPropertyOf owl:topDataProperty ;
                    rdfs:comment "A detailed description of the Process Control Automation System, including its capabilities, components, and the specific processes it controls." .


###  http://WSP.org/ontology/cro#PCASName
cro:PCASName rdf:type owl:DatatypeProperty ;
             rdfs:comment "The official name or designation of the Process Control Automation System, used for identification and documentation purposes." .


###  http://WSP.org/ontology/cro#PCASlocatedIn
cro:PCASlocatedIn rdf:type owl:DatatypeProperty ;
                  rdfs:comment "The physical location where the Process Control Automation System is installed, such as a control room, facility, or specific site within an operation." .


###  http://WSP.org/ontology/cro#ShipsMaterialTo
cro:ShipsMaterialTo rdf:type owl:DatatypeProperty ;
                    rdfs:comment "Specifies the destination to which materials are shipped or transported from a facility or terminal." .


###  http://WSP.org/ontology/cro#TSFCapacity
cro:TSFCapacity rdf:type owl:DatatypeProperty .


###  http://WSP.org/ontology/cro#TSFConsequenceCategory
cro:TSFConsequenceCategory rdf:type owl:DatatypeProperty .


###  http://WSP.org/ontology/cro#TSFName
cro:TSFName rdf:type owl:DatatypeProperty .


###  http://WSP.org/ontology/cro#TSFStatus
cro:TSFStatus rdf:type owl:DatatypeProperty .


###  http://WSP.org/ontology/cro#Tsunami
cro:Tsunami rdf:type owl:DatatypeProperty ;
            rdfs:comment "Indicates the tsunami risk or history for a specific location, relevant to disaster planning and risk assessment." .


###  http://WSP.org/ontology/cro#agedConditionBoolean
cro:agedConditionBoolean rdf:type owl:DatatypeProperty ;
                         rdfs:comment "Indicates whether the equipment or facility is considered to be in an aged or worn condition, which may impact its reliability or performance." .


###  http://WSP.org/ontology/cro#amountOfEquipmentAvailable
cro:amountOfEquipmentAvailable rdf:type owl:DatatypeProperty ;
                               rdfs:comment "The quantity of equipment of the specificed individual available within a facility or operation, often important for resource management." .


###  http://WSP.org/ontology/cro#amperage
cro:amperage rdf:type owl:DatatypeProperty ;
             rdfs:comment "Represents the current in amperes (A) carried by the transmission lines or transformers." .


###  http://WSP.org/ontology/cro#appointmentDate
cro:appointmentDate rdf:type owl:DatatypeProperty .


###  http://WSP.org/ontology/cro#assetGroup
cro:assetGroup rdf:type owl:DatatypeProperty ;
               rdfs:range xsd:string ;
               rdfs:comment "Represents the asset group involved in a critical risk scenario." ,
                            "The group of assets associated with the risk scenario." .


###  http://WSP.org/ontology/cro#assumptionDescription
cro:assumptionDescription rdf:type owl:DatatypeProperty .


###  http://WSP.org/ontology/cro#auditAndReviewDescription
cro:auditAndReviewDescription rdf:type owl:DatatypeProperty ;
                              rdfs:comment "A detailed description of the audit or review, including its scope, findings, and recommendations." .


###  http://WSP.org/ontology/cro#auditReviewName
cro:auditReviewName rdf:type owl:DatatypeProperty ;
                    rdfs:comment "The name or title of a specific audit or review conducted as part of the assessment process." .


###  http://WSP.org/ontology/cro#benchHeight
cro:benchHeight rdf:type owl:DatatypeProperty ;
                rdfs:range xsd:decimal .


###  http://WSP.org/ontology/cro#bermWidth
cro:bermWidth rdf:type owl:DatatypeProperty .


###  http://WSP.org/ontology/cro#berthName
cro:berthName rdf:type owl:DatatypeProperty ;
              rdfs:comment "The name or designation of a berth within a port, used to identify specific docking locations." .


###  http://WSP.org/ontology/cro#berthTerminal
cro:berthTerminal rdf:type owl:DatatypeProperty ;
                  rdfs:comment "The terminal associated with a specific berth, used in port and marine operations." .


###  http://WSP.org/ontology/cro#businessInterruptionUSDM
cro:businessInterruptionUSDM rdf:type owl:DatatypeProperty ;
                             rdfs:comment "Represents the business interruption loss in USD from a critical risk scenario." .


###  http://WSP.org/ontology/cro#capacity
cro:capacity rdf:type owl:DatatypeProperty .


###  http://WSP.org/ontology/cro#catastrophicRiskScenariowithLowProbability
cro:catastrophicRiskScenariowithLowProbability rdf:type owl:DatatypeProperty ;
                                               rdfs:comment "Individual examples or illustrations of catastrophic risk scenarios with low probability" .


###  http://WSP.org/ontology/cro#cellNumber
cro:cellNumber rdf:type owl:DatatypeProperty .


###  http://WSP.org/ontology/cro#cellStatus
cro:cellStatus rdf:type owl:DatatypeProperty .


###  http://WSP.org/ontology/cro#changeDescription
cro:changeDescription rdf:type owl:DatatypeProperty ;
                      rdfs:comment "Describe wether  the change in terms of an Organiational Change, a system change, a change to raw materials, production or sales, a change to equipment and facilities, a change to external environment or a change to a specific sritical risk scenario." .


###  http://WSP.org/ontology/cro#changeInBusinessInterruption
cro:changeInBusinessInterruption rdf:type owl:DatatypeProperty ;
                                 rdfs:comment "Indicates changes in the risk or impact of business interruptions, often related to new mitigation strategies or incidents." .


###  http://WSP.org/ontology/cro#changeInEnvironment
cro:changeInEnvironment rdf:type owl:DatatypeProperty ;
                        rdfs:comment "Indicates whether there has been a significant change in the environment affecting the operation." .


###  http://WSP.org/ontology/cro#changeInEnvironmentDescription
cro:changeInEnvironmentDescription rdf:type owl:DatatypeProperty ;
                                   rdfs:comment "Describes changes in the external or internal environment, such as regulatory shifts, climate changes, or operational impacts." .


###  http://WSP.org/ontology/cro#changeInPortDescription
cro:changeInPortDescription rdf:type owl:DatatypeProperty ;
                            rdfs:comment "Describes modifications or updates that have occurred at the port, including infrastructure changes or operational adjustments." .


###  http://WSP.org/ontology/cro#changeInProduction
cro:changeInProduction rdf:type owl:DatatypeProperty ;
                       rdfs:comment "Describes changes in production volumes, methods, or outputs, often in response to operational changes or market demand." .


###  http://WSP.org/ontology/cro#changeInRawMaterial
cro:changeInRawMaterial rdf:type owl:DatatypeProperty ;
                        rdfs:comment "Indicates changes in the raw materials used, including changes in supply, type, or quality." .


###  http://WSP.org/ontology/cro#changeInSales
cro:changeInSales rdf:type owl:DatatypeProperty ;
                  rdfs:comment "Records changes in sales figures or projections, often linked to changes in production or market conditions." .


###  http://WSP.org/ontology/cro#changeName
cro:changeName rdf:type owl:DatatypeProperty ;
               rdfs:comment "Identifies wether the change is an Organiational Change, a system change, a change to raw materials, production or sales, a change to equipment and facilities, a change to external environment or a change to a specific sritical risk scenario." .


###  http://WSP.org/ontology/cro#checkedBy
cro:checkedBy rdf:type owl:DatatypeProperty ;
              rdfs:comment "Specifies the individual or entity responsible for reviewing and verifying a document, report, or process." .


###  http://WSP.org/ontology/cro#classification
cro:classification rdf:type owl:DatatypeProperty ;
                   rdfs:comment "Represents the classification of a recommendation." .


###  http://WSP.org/ontology/cro#completeRecommendationNumber
cro:completeRecommendationNumber rdf:type owl:DatatypeProperty ;
                                 rdfs:comment "Represents the number of completed recommendations." .


###  http://WSP.org/ontology/cro#constructionMethod
cro:constructionMethod rdf:type owl:DatatypeProperty .


###  http://WSP.org/ontology/cro#contactDescription
cro:contactDescription rdf:type owl:DatatypeProperty ;
                       rdfs:comment "Discussions and/or inspections took place on site with the following personnel" .


###  http://WSP.org/ontology/cro#contactName
cro:contactName rdf:type owl:DatatypeProperty .


###  http://WSP.org/ontology/cro#contactRole
cro:contactRole rdf:type owl:DatatypeProperty .


###  http://WSP.org/ontology/cro#criticaRiskScenarioDefinition
cro:criticaRiskScenarioDefinition rdf:type owl:DatatypeProperty ;
                                  rdfs:comment "The definition of a Critical Risk Scenario as stated by the CRA Report." .


###  http://WSP.org/ontology/cro#criticalRiskScenarioChangeFromPrevious
cro:criticalRiskScenarioChangeFromPrevious rdf:type owl:DatatypeProperty ;
                                           rdfs:comment "States what changed in the Critical Risk Scenario in comparisson to the previous one, highlighting any updates or modifications." .


###  http://WSP.org/ontology/cro#criticalRiskScenarioID
cro:criticalRiskScenarioID rdf:type owl:DatatypeProperty ;
                           rdfs:subPropertyOf owl:topDataProperty ;
                           rdfs:comment "A unique identifier for each critical risk scenario, used for tracking and reference purposes, such as \"DPO-##\"" ,
                                        "The Identification number or ID for the critical risk scenario. Normally an acronym follower by a number. For Dampier Port, the IDs are: DPO-##" .


###  http://WSP.org/ontology/cro#currentSurveyRatingSummaryPercentage
cro:currentSurveyRatingSummaryPercentage rdf:type owl:DatatypeProperty .


###  http://WSP.org/ontology/cro#currentSurveySubElementScore
cro:currentSurveySubElementScore rdf:type owl:DatatypeProperty .


###  http://WSP.org/ontology/cro#currentSurveySystemPercentage
cro:currentSurveySystemPercentage rdf:type owl:DatatypeProperty .


###  http://WSP.org/ontology/cro#dateCompletedSupersededRejected
cro:dateCompletedSupersededRejected rdf:type owl:DatatypeProperty ;
                                    rdfs:comment "Represents the date a recommendation was completed, suspended, or rejected." .


###  http://WSP.org/ontology/cro#dependencyDefinition
cro:dependencyDefinition rdf:type owl:DatatypeProperty ;
                         rdfs:comment "The various dependencies of the site on external providers have been considered." .


###  http://WSP.org/ontology/cro#designCapacity
cro:designCapacity rdf:type owl:DatatypeProperty .


###  http://WSP.org/ontology/cro#designDate
cro:designDate rdf:type owl:DatatypeProperty .


###  http://WSP.org/ontology/cro#designMaterialSpecification
cro:designMaterialSpecification rdf:type owl:DatatypeProperty ;
                                rdfs:comment "The materials and design specifications used in the construction of the transmission lines or substations, ensuring they meet required standards." .


###  http://WSP.org/ontology/cro#dimensions
cro:dimensions rdf:type owl:DatatypeProperty .


###  http://WSP.org/ontology/cro#distributionSystemDescription
cro:distributionSystemDescription rdf:type owl:DatatypeProperty ;
                                  rdfs:comment "A description of the distribution system in the electrical network." .


###  http://WSP.org/ontology/cro#distributionSystemName
cro:distributionSystemName rdf:type owl:DatatypeProperty ;
                           rdfs:comment "The name assigned to the distribution system in the network." .


###  http://WSP.org/ontology/cro#divisionDescription
cro:divisionDescription rdf:type owl:DatatypeProperty ;
                        rdfs:comment "A detailed description of the division within a company, outlining its responsibilities, scope of work, and key objectives." .


###  http://WSP.org/ontology/cro#dredgeDepth
cro:dredgeDepth rdf:type owl:DatatypeProperty ;
                rdfs:comment "The depth to which a berth or channel has been dredged, important for determining vessel accommodation." .


###  http://WSP.org/ontology/cro#earthquakeZone
cro:earthquakeZone rdf:type owl:DatatypeProperty ;
                   rdfs:comment "Indicates the earthquake zone classification for a given location, used in risk assessments." .


###  http://WSP.org/ontology/cro#electricityDemand
cro:electricityDemand rdf:type owl:DatatypeProperty ;
                      rdfs:comment "The amount of electricity required by a process or location to operate effectively, typically measured in kilowatts or megawatts." .


###  http://WSP.org/ontology/cro#embankmentHeight
cro:embankmentHeight rdf:type owl:DatatypeProperty .


###  http://WSP.org/ontology/cro#embankmentLength
cro:embankmentLength rdf:type owl:DatatypeProperty .


###  http://WSP.org/ontology/cro#engineCapacity
cro:engineCapacity rdf:type owl:DatatypeProperty ;
                   rdfs:comment "Represents the capacity of the engine, usually in terms of power output." .


###  http://WSP.org/ontology/cro#engineModel
cro:engineModel rdf:type owl:DatatypeProperty ;
                rdfs:comment "The specific model of the engine used in turbines or generators." .


###  http://WSP.org/ontology/cro#equipmentChangeDescription
cro:equipmentChangeDescription rdf:type owl:DatatypeProperty ;
                               rdfs:comment "A detailed description of the changes made to equipment, including replacements, upgrades, or maintenance." .


###  http://WSP.org/ontology/cro#equipmentChanged
cro:equipmentChanged rdf:type owl:DatatypeProperty ;
                     rdfs:comment "Indicates what secific equipment has undergone a change since the last assessment." .


###  http://WSP.org/ontology/cro#equipmentDescription
cro:equipmentDescription rdf:type owl:DatatypeProperty ;
                         rdfs:comment "A description of the equipment, including its function, specifications, and operational context." .


###  http://WSP.org/ontology/cro#equipmentName
cro:equipmentName rdf:type owl:DatatypeProperty ;
                  rdfs:comment "The designated name of the equipment, used within inventory systems to track and manage assets." .


###  http://WSP.org/ontology/cro#equipmentReplacedDate
cro:equipmentReplacedDate rdf:type owl:DatatypeProperty ;
                          rdfs:comment "The date on which the equipment was replaced, used for maintenance records and lifecycle management." .


###  http://WSP.org/ontology/cro#equipmentType
cro:equipmentType rdf:type owl:DatatypeProperty ;
                  rdfs:comment "Type of Equipment refers to what kind of equipment the individual is: Car, Vessel, etc" .


###  http://WSP.org/ontology/cro#estimatedCost
cro:estimatedCost rdf:type owl:DatatypeProperty ;
                  rdfs:comment "The estimated cost of implementing the recommendation." .


###  http://WSP.org/ontology/cro#expectedFailureDate
cro:expectedFailureDate rdf:type owl:DatatypeProperty .


###  http://WSP.org/ontology/cro#expenditure
cro:expenditure rdf:type owl:DatatypeProperty ;
                rdfs:comment "Represents the expenditure related to a recommendation." .


###  http://WSP.org/ontology/cro#extratropicalCycloner
cro:extratropicalCycloner rdf:type owl:DatatypeProperty .


###  http://WSP.org/ontology/cro#facilityChangeDescription
cro:facilityChangeDescription rdf:type owl:DatatypeProperty ;
                              rdfs:comment "A description of the changes made to a facility, such as upgrades, repairs, or modifications." .


###  http://WSP.org/ontology/cro#facilityChanged
cro:facilityChanged rdf:type owl:DatatypeProperty ;
                    rdfs:comment "Indicates what specific facility has undergone significant changes since the last assessment." .


###  http://WSP.org/ontology/cro#facilityDescription
cro:facilityDescription rdf:type owl:DatatypeProperty ;
                        rdfs:comment "A detailed description of the facility, outlining its purpose, operations, and key features." .


###  http://WSP.org/ontology/cro#facilityName
cro:facilityName rdf:type owl:DatatypeProperty ;
                 rdfs:comment "The name of the facility, identifying it within the operation." .


###  http://WSP.org/ontology/cro#finalProductDescription
cro:finalProductDescription rdf:type owl:DatatypeProperty .


###  http://WSP.org/ontology/cro#fireSupressionCondition
cro:fireSupressionCondition rdf:type owl:DatatypeProperty ;
                            rdfs:comment "The current state or condition of the fire suppression systems within the substation, critical for ensuring safety and compliance." .


###  http://WSP.org/ontology/cro#flood
cro:flood rdf:type owl:DatatypeProperty ;
          rdfs:comment "Indicates the flood risk or history for a specific location, used in environmental and risk assessments." .


###  http://WSP.org/ontology/cro#generalInformationDescription
cro:generalInformationDescription rdf:type owl:DatatypeProperty .


###  http://WSP.org/ontology/cro#generalNotes
cro:generalNotes rdf:type owl:DatatypeProperty ;
                 rdfs:comment "General information about SURVEY AND REPORT DETAILS, such as abbreviations, estimated time periods, etc." .


###  http://WSP.org/ontology/cro#generatorCapacity
cro:generatorCapacity rdf:type owl:DatatypeProperty ;
                      rdfs:comment "The maximum electrical output capacity of a generator." .


###  http://WSP.org/ontology/cro#grade
cro:grade rdf:type owl:DatatypeProperty .


###  http://WSP.org/ontology/cro#hardControls
cro:hardControls rdf:type owl:DatatypeProperty .


###  http://WSP.org/ontology/cro#hasAddress
cro:hasAddress rdf:type owl:DatatypeProperty ;
               rdfs:comment "The physical address of the operation or facility, used for location and correspondence purposes." .


###  http://WSP.org/ontology/cro#hasBusiness
cro:hasBusiness rdf:type owl:DatatypeProperty ;
                rdfs:comment "Describes the nature or type of business conducted by a company, such as manufacturing, consulting, or logistics." .


###  http://WSP.org/ontology/cro#hasCRADate
cro:hasCRADate rdf:type owl:DatatypeProperty ;
               rdfs:comment "The date when the Critical Risk Assessment (CRA) was created or last updated." .


###  http://WSP.org/ontology/cro#hasCRAType
cro:hasCRAType rdf:type owl:DatatypeProperty ;
               rdfs:comment "Specifies the type of Critical Risk Assessment (CRA), such as MFL, NLE, etc" ,
                            "Specifies the type of Critical Risk Assessment (CRA), such as a safety or environmental risk assessment." .


###  http://WSP.org/ontology/cro#hasCompanyName
cro:hasCompanyName rdf:type owl:DatatypeProperty ;
                   rdfs:comment "The official name of the company, used for identification and legal purposes." .


###  http://WSP.org/ontology/cro#hasDate
cro:hasDate rdf:type owl:DatatypeProperty ;
            rdfs:comment "A general date property, used to capture important dates related to incidents, changes, or assessments." .


###  http://WSP.org/ontology/cro#hasDateOfIssue
cro:hasDateOfIssue rdf:type owl:DatatypeProperty ;
                   rdfs:comment "The date on which a document, report, or directive was officially issued." .


###  http://WSP.org/ontology/cro#hasDateOfSurvey
cro:hasDateOfSurvey rdf:type owl:DatatypeProperty ;
                    rdfs:comment "The date on which the survey or assessment was conducted, typically associated with a Critical Risk Assessment (CRA)." ,
                                 "The date on which the survey or assessment was conducted." .


###  http://WSP.org/ontology/cro#hasEmail
cro:hasEmail rdf:type owl:DatatypeProperty ;
             rdfs:comment "The email address of an employee, used for communication within the company." .


###  http://WSP.org/ontology/cro#hasEmployeeEmail
cro:hasEmployeeEmail rdf:type owl:DatatypeProperty ;
                     rdfs:comment "The email address of an employee, used for communication within the company." .


###  http://WSP.org/ontology/cro#hasEmployeePhoneNumber
cro:hasEmployeePhoneNumber rdf:type owl:DatatypeProperty ;
                           rdfs:comment "The phone number of an employee, used for contact and communication within the company." .


###  http://WSP.org/ontology/cro#hasFirstName
cro:hasFirstName rdf:type owl:DatatypeProperty ;
                 rdfs:comment "The first name of an employee, used for identification within the company." .


###  http://WSP.org/ontology/cro#hasLastName
cro:hasLastName rdf:type owl:DatatypeProperty ;
                rdfs:comment "The last name of an employee, used for identification within the company." .


###  http://WSP.org/ontology/cro#hasLatitude
cro:hasLatitude rdf:type owl:DatatypeProperty ;
                rdfs:comment "The geographic latitude of the facility or operation, used for mapping and location purposes." .


###  http://WSP.org/ontology/cro#hasLongitude
cro:hasLongitude rdf:type owl:DatatypeProperty ;
                 rdfs:comment "The geographic longitude of the facility or operation, used for mapping and location purposes." .


###  http://WSP.org/ontology/cro#hasName
cro:hasName rdf:type owl:DatatypeProperty .


###  http://WSP.org/ontology/cro#hasPhone
cro:hasPhone rdf:type owl:DatatypeProperty ;
             rdfs:comment "The contact phone number associated with the Process Control Automation System, typically used for support or emergency contact." ,
                          "The phone number associated with the operation, facility, or division, used for contact purposes." .


###  http://WSP.org/ontology/cro#hasRevisionDetail
cro:hasRevisionDetail rdf:type owl:DatatypeProperty ;
                      rdfs:comment "The details associated with the revision of a document, report, or assessment, outlining what changes or updates were made." .


###  http://WSP.org/ontology/cro#highReturnNewRecommendations
cro:highReturnNewRecommendations rdf:type owl:DatatypeProperty ;
                                 rdfs:comment "Represents the number of new recommendations with a high return." .


###  http://WSP.org/ontology/cro#inProgressRecommendationNumber
cro:inProgressRecommendationNumber rdf:type owl:DatatypeProperty ;
                                   rdfs:comment "Represents the number of recommendations that are currently in progress." .


###  http://WSP.org/ontology/cro#incidentDescription
cro:incidentDescription rdf:type owl:DatatypeProperty ;
                        rdfs:subPropertyOf owl:topDataProperty ;
                        rdfs:comment "A narrative description of a specific incident, including what occurred, its impact, and any resulting actions." ,
                                     "Provides a detailed description of the incident." .


###  http://WSP.org/ontology/cro#incidentName
cro:incidentName rdf:type owl:DatatypeProperty ;
                 rdfs:comment "The name or title given to a specific incident, used for identification and tracking purposes." .


###  http://WSP.org/ontology/cro#incidentSummary
cro:incidentSummary rdf:type owl:DatatypeProperty ;
                    rdfs:range xsd:string ;
                    rdfs:comment "A summary of the incident in the critical risk scenario." ,
                                 "Contains a summary of an incident in a critical risk scenario." .


###  http://WSP.org/ontology/cro#incrementalImprovementNumber
cro:incrementalImprovementNumber rdf:type owl:DatatypeProperty ;
                                 rdfs:comment "Represents the number of incremental improvements." .


###  http://WSP.org/ontology/cro#inherentControls
cro:inherentControls rdf:type owl:DatatypeProperty .


###  http://WSP.org/ontology/cro#inherentHazards
cro:inherentHazards rdf:type owl:DatatypeProperty .


###  http://WSP.org/ontology/cro#inloadingDescription
cro:inloadingDescription rdf:type owl:DatatypeProperty ;
                         rdfs:comment "A description of the inloading process, detailing how materials are dispatched from the facility." .


###  http://WSP.org/ontology/cro#inloadsMaterialFrom
cro:inloadsMaterialFrom rdf:type owl:DatatypeProperty ;
                        rdfs:comment "Indicates the source of materials being inloaded into the facility or terminal." .


###  http://WSP.org/ontology/cro#inputVoltage
cro:inputVoltage rdf:type owl:DatatypeProperty ;
                 rdfs:comment "Represents the input and output voltage of transformers or other electrical components." .


###  http://WSP.org/ontology/cro#installationDate
cro:installationDate rdf:type owl:DatatypeProperty ;
                     rdfs:comment "The date when a particular component, such as a transmission line or transformer, was installed." .


###  http://WSP.org/ontology/cro#likelihood
cro:likelihood rdf:type owl:DatatypeProperty ;
               rdfs:range xsd:string ;
               rdfs:comment "Likelihood of the critical risk scenario occurring." ,
                            "Represents the likelihood of a critical risk scenario occurring." ,
                            "The likelihood of the recommendation's success." .


###  http://WSP.org/ontology/cro#likelihoodAfterRecommendation
cro:likelihoodAfterRecommendation rdf:type owl:DatatypeProperty .


###  http://WSP.org/ontology/cro#likelihoodNow
cro:likelihoodNow rdf:type owl:DatatypeProperty .


###  http://WSP.org/ontology/cro#lossEstimateAfterRecommendationUSDM
cro:lossEstimateAfterRecommendationUSDM rdf:type owl:DatatypeProperty ;
                                        rdfs:comment "Represents the loss estimate after the recommendation in USD." .


###  http://WSP.org/ontology/cro#lossEstimateNowUSDM
cro:lossEstimateNowUSDM rdf:type owl:DatatypeProperty ;
                        rdfs:comment "Represents the current loss estimate in USD." .


###  http://WSP.org/ontology/cro#lossScenarioPeril
cro:lossScenarioPeril rdf:type owl:DatatypeProperty ;
                      rdfs:range xsd:string ;
                      rdfs:comment "Peril or hazard causing the loss." ,
                                   "Represents the peril associated with a loss scenario." .


###  http://WSP.org/ontology/cro#lossUsdm
cro:lossUsdm rdf:type owl:DatatypeProperty ;
             rdfs:comment "The loss in USD millions associated with the recommendation." .


###  http://WSP.org/ontology/cro#mandarotyNewRecommendations
cro:mandarotyNewRecommendations rdf:type owl:DatatypeProperty .


###  http://WSP.org/ontology/cro#materialHandled
cro:materialHandled rdf:type owl:DatatypeProperty ;
                    rdfs:comment "Describes the type of material handled by the facility or terminal, such as ore, grain, or liquid cargo." .


###  http://WSP.org/ontology/cro#materialHandledAmount
cro:materialHandledAmount rdf:type owl:DatatypeProperty ;
                          rdfs:comment "The quantity of material handled by a facility or terminal, typically measured in tons or similar units." .


###  http://WSP.org/ontology/cro#mediumReturnNewRecommendations
cro:mediumReturnNewRecommendations rdf:type owl:DatatypeProperty ;
                                   rdfs:comment "Represents the number of new recommendations with a medium return." .


###  http://WSP.org/ontology/cro#mineLocation
cro:mineLocation rdf:type owl:DatatypeProperty .


###  http://WSP.org/ontology/cro#mineName
cro:mineName rdf:type owl:DatatypeProperty .


###  http://WSP.org/ontology/cro#mineType
cro:mineType rdf:type owl:DatatypeProperty .


###  http://WSP.org/ontology/cro#networkDescription
cro:networkDescription rdf:type owl:DatatypeProperty ;
                       rdfs:comment "A description of the overall power network and its components." .


###  http://WSP.org/ontology/cro#networkName
cro:networkName rdf:type owl:DatatypeProperty ;
                rdfs:comment "The name of the power network." .


###  http://WSP.org/ontology/cro#numberOfContractors
cro:numberOfContractors rdf:type owl:DatatypeProperty ;
                        rdfs:comment "Specifies the number of contractors involved in an operation or project, providing insight into the scale of external workforce involvement." .


###  http://WSP.org/ontology/cro#numberOfEmployees
cro:numberOfEmployees rdf:type owl:DatatypeProperty .


###  http://WSP.org/ontology/cro#numberOfPanels
cro:numberOfPanels rdf:type owl:DatatypeProperty .


###  http://WSP.org/ontology/cro#numberOfShafts
cro:numberOfShafts rdf:type owl:DatatypeProperty .


###  http://WSP.org/ontology/cro#operationCriticalReliance
cro:operationCriticalReliance rdf:type owl:DatatypeProperty ;
                              rdfs:comment "Indicates the degree to which an operation relies on a specific substation or transmission line, particularly in terms of critical load and redundancy." .


###  http://WSP.org/ontology/cro#operationDescription
cro:operationDescription rdf:type owl:DatatypeProperty ;
                         rdfs:comment "A detailed description of the operation, covering its scope, activities, and objectives." .


###  http://WSP.org/ontology/cro#oreBodyName
cro:oreBodyName rdf:type owl:DatatypeProperty .


###  http://WSP.org/ontology/cro#oreTypeProcessed
cro:oreTypeProcessed rdf:type owl:DatatypeProperty .


###  http://WSP.org/ontology/cro#organisationalChangeDescription
cro:organisationalChangeDescription rdf:type owl:DatatypeProperty ;
                                    rdfs:comment "A narrative detailing the changes in the organizational structure, such as new appointments or reorganization." .


###  http://WSP.org/ontology/cro#otherCostsUSDM
cro:otherCostsUSDM rdf:type owl:DatatypeProperty ;
                   rdfs:comment "Represents other costs in USD from a critical risk scenario." .


###  http://WSP.org/ontology/cro#otherDependenciesDescription
cro:otherDependenciesDescription rdf:type owl:DatatypeProperty .


###  http://WSP.org/ontology/cro#outloadingDescription
cro:outloadingDescription rdf:type owl:DatatypeProperty ;
                          rdfs:comment "A description of the outloading process, detailing how materials are dispatched from the facility." .


###  http://WSP.org/ontology/cro#outloadsMaterialTo
cro:outloadsMaterialTo rdf:type owl:DatatypeProperty ;
                       rdfs:comment "Specifies the destination to which materials are outloaded from the facility or terminal." .


###  http://WSP.org/ontology/cro#outputVoltage
cro:outputVoltage rdf:type owl:DatatypeProperty ;
                  rdfs:comment "The voltage output by a transformer or generator." .


###  http://WSP.org/ontology/cro#portName
cro:portName rdf:type owl:DatatypeProperty ;
             rdfs:comment "The name of the port, used to identify the specific port within broader operations." .


###  http://WSP.org/ontology/cro#positionAccountable
cro:positionAccountable rdf:type owl:DatatypeProperty ;
                        rdfs:comment "Represents the accountable position for a recommendation." .


###  http://WSP.org/ontology/cro#powerDemand
cro:powerDemand rdf:type owl:DatatypeProperty ;
                rdfs:comment "Indicates the amount of power required by a facility, process, or operation, typically measured in kilowatts or megawatts." .


###  http://WSP.org/ontology/cro#powerStationCapacity
cro:powerStationCapacity rdf:type owl:DatatypeProperty ;
                         rdfs:comment "The electrical capacity of the power station, typically in megawatts (MW)." .


###  http://WSP.org/ontology/cro#powerStationDescription
cro:powerStationDescription rdf:type owl:DatatypeProperty ;
                            rdfs:comment "A description of the power station and its components." .


###  http://WSP.org/ontology/cro#powerStationLocation
cro:powerStationLocation rdf:type owl:DatatypeProperty ;
                         rdfs:comment "The physical location of the power station." .


###  http://WSP.org/ontology/cro#powerStationName
cro:powerStationName rdf:type owl:DatatypeProperty ;
                     rdfs:comment "The name assigned to the power station." .


###  http://WSP.org/ontology/cro#powerStationType
cro:powerStationType rdf:type owl:DatatypeProperty ;
                     rdfs:comment "The type of the power station, such as gas-powered or diesel-powered." .


###  http://WSP.org/ontology/cro#preincident_and_workaroundARP
cro:preincident_and_workaroundARP rdf:type owl:DatatypeProperty .


###  http://WSP.org/ontology/cro#previousSurveyRatingSummaryPercentage
cro:previousSurveyRatingSummaryPercentage rdf:type owl:DatatypeProperty .


###  http://WSP.org/ontology/cro#previousSurveySubElementScore
cro:previousSurveySubElementScore rdf:type owl:DatatypeProperty .


###  http://WSP.org/ontology/cro#previousSurveySystemPercentage
cro:previousSurveySystemPercentage rdf:type owl:DatatypeProperty .


###  http://WSP.org/ontology/cro#priority
cro:priority rdf:type owl:DatatypeProperty ;
             rdfs:comment "The priority level of the recommendation." .


###  http://WSP.org/ontology/cro#processDescription
cro:processDescription rdf:type owl:DatatypeProperty ;
                       rdfs:comment "A detailed description of a specific process within a facility or operation, outlining the steps, objectives, and key activities involved." .


###  http://WSP.org/ontology/cro#projectCompletionDate
cro:projectCompletionDate rdf:type owl:DatatypeProperty ;
                          rdfs:comment "The anticipated or actual date when the Project is expected to be completed." .


###  http://WSP.org/ontology/cro#projectDescription
cro:projectDescription rdf:type owl:DatatypeProperty ;
                       rdfs:comment "A detailed narrative describing the scope, objectives, and key components of the Project." .


###  http://WSP.org/ontology/cro#projectName
cro:projectName rdf:type owl:DatatypeProperty ;
                rdfs:comment "Name of the project" .


###  http://WSP.org/ontology/cro#propertyDamageUSDM
cro:propertyDamageUSDM rdf:type owl:DatatypeProperty ;
                       rdfs:comment "Represents the property damage in USD from a critical risk scenario." .


###  http://WSP.org/ontology/cro#rawMaterialDescription
cro:rawMaterialDescription rdf:type owl:DatatypeProperty ;
                           rdfs:comment "Description of any raw material the site is dependent upon." .


###  http://WSP.org/ontology/cro#rawMaterialName
cro:rawMaterialName rdf:type owl:DatatypeProperty ;
                    rdfs:comment "Name of any raw material the site is dependent upon." .


###  http://WSP.org/ontology/cro#recievesMaterialFrom
cro:recievesMaterialFrom rdf:type owl:DatatypeProperty ;
                         rdfs:comment "Specifies the source from which the facility or terminal receives materials, such as another facility or port." .


###  http://WSP.org/ontology/cro#recommendationDefinition
cro:recommendationDefinition rdf:type owl:DatatypeProperty .


###  http://WSP.org/ontology/cro#recommendationDescription
cro:recommendationDescription rdf:type owl:DatatypeProperty ;
                              rdfs:comment "The description of a recommendation for a Critical Risk Scenario." .


###  http://WSP.org/ontology/cro#recommendationDetailText
cro:recommendationDetailText rdf:type owl:DatatypeProperty ;
                             rdfs:comment "Contains the detailed description of a recommendation." .


###  http://WSP.org/ontology/cro#recommendationEstimatedCostUSDM
cro:recommendationEstimatedCostUSDM rdf:type owl:DatatypeProperty ;
                                    rdfs:comment "Represents the estimated cost of a recommendation." .


###  http://WSP.org/ontology/cro#recommendationImprovement
cro:recommendationImprovement rdf:type owl:DatatypeProperty ;
                              rdfs:comment "Represents the improvement made by a recommendation." .


###  http://WSP.org/ontology/cro#recommendationPriority
cro:recommendationPriority rdf:type owl:DatatypeProperty .


###  http://WSP.org/ontology/cro#recommendationStatus
cro:recommendationStatus rdf:type owl:DatatypeProperty .


###  http://WSP.org/ontology/cro#recommendationYear
cro:recommendationYear rdf:type owl:DatatypeProperty ;
                       rdfs:comment "Represents the year the recommendation was made." .


###  http://WSP.org/ontology/cro#recommendationsCompletedSinceLastReview
cro:recommendationsCompletedSinceLastReview rdf:type owl:DatatypeProperty .


###  http://WSP.org/ontology/cro#recoveryRepair
cro:recoveryRepair rdf:type owl:DatatypeProperty ;
                   rdfs:comment "Describes the recovery or repair process after an incident." .


###  http://WSP.org/ontology/cro#referenceDocumentDescription
cro:referenceDocumentDescription rdf:type owl:DatatypeProperty .


###  http://WSP.org/ontology/cro#referenceNumber
cro:referenceNumber rdf:type owl:DatatypeProperty ;
                    rdfs:comment "The reference number for the recommendation." .


###  http://WSP.org/ontology/cro#region
cro:region rdf:type owl:DatatypeProperty ;
           rdfs:comment "The geographical region where the power network or component is located." .


###  http://WSP.org/ontology/cro#rejectedRecommendationDescription
cro:rejectedRecommendationDescription rdf:type owl:DatatypeProperty ;
                                      rdfs:comment "Represents the description of a rejected recommendation." .


###  http://WSP.org/ontology/cro#rejectedRecommendationNumber
cro:rejectedRecommendationNumber rdf:type owl:DatatypeProperty ;
                                 rdfs:comment "Represents the number of rejected recommendations." .


###  http://WSP.org/ontology/cro#repairPeriod
cro:repairPeriod rdf:type owl:DatatypeProperty ;
                 rdfs:comment "Represents the repair period duration after an incident." .


###  http://WSP.org/ontology/cro#retiredInYear
cro:retiredInYear rdf:type owl:DatatypeProperty ;
                  rdfs:comment "The year in which the Process Control Automation System or its components were decommissioned or retired from active service." .


###  http://WSP.org/ontology/cro#riskLikelihoodClassification
cro:riskLikelihoodClassification rdf:type owl:DatatypeProperty ;
                                 rdfs:comment "The likelihood of the risks has been assigned one of five classifications; “Almost Certain”, “Likely”, “Possible”, “Unlikely”, “Rare”." .


###  http://WSP.org/ontology/cro#riskManagementSubElementInformation
cro:riskManagementSubElementInformation rdf:type owl:DatatypeProperty .


###  http://WSP.org/ontology/cro#runByDieselBoolean
cro:runByDieselBoolean rdf:type owl:DatatypeProperty ;
                       rdfs:comment "Indicates whether the engine runs on diesel (yes/no)." .


###  http://WSP.org/ontology/cro#runByGasBoolean
cro:runByGasBoolean rdf:type owl:DatatypeProperty ;
                    rdfs:comment "Indicates whether the engine runs on natural gas (yes/no)." .


###  http://WSP.org/ontology/cro#shape
cro:shape rdf:type owl:DatatypeProperty .


###  http://WSP.org/ontology/cro#significantChangeDescription
cro:significantChangeDescription rdf:type owl:DatatypeProperty .


###  http://WSP.org/ontology/cro#siteResponseOrComments
cro:siteResponseOrComments rdf:type owl:DatatypeProperty ;
                           rdfs:comment "Contains the site's response or comments on the recommendation." .


###  http://WSP.org/ontology/cro#slopeAngle
cro:slopeAngle rdf:type owl:DatatypeProperty .


###  http://WSP.org/ontology/cro#softControls
cro:softControls rdf:type owl:DatatypeProperty .


###  http://WSP.org/ontology/cro#spillwayStatus
cro:spillwayStatus rdf:type owl:DatatypeProperty .


###  http://WSP.org/ontology/cro#status
cro:status rdf:type owl:DatatypeProperty ;
           rdfs:comment "The current status of the recommendation." .


###  http://WSP.org/ontology/cro#stockpileCapacity
cro:stockpileCapacity rdf:type owl:DatatypeProperty .


###  http://WSP.org/ontology/cro#stormSurge
cro:stormSurge rdf:type owl:DatatypeProperty ;
               rdfs:comment "Indicates the risk or history of storm surges at a specific location, relevant for disaster planning and coastal risk assessments." .


###  http://WSP.org/ontology/cro#subFacilityDescription
cro:subFacilityDescription rdf:type owl:DatatypeProperty ;
                           rdfs:comment "A detailed description of a sub-facility within a larger operation, outlining its specific role and functions." .


###  http://WSP.org/ontology/cro#subFacilityName
cro:subFacilityName rdf:type owl:DatatypeProperty ;
                    rdfs:comment "The name assigned to a sub-facility, distinguishing it within the broader operation.\"" .


###  http://WSP.org/ontology/cro#substationCondition
cro:substationCondition rdf:type owl:DatatypeProperty ;
                        rdfs:comment "The current condition of the substation (e.g., good, needs repair)." .


###  http://WSP.org/ontology/cro#substationDescription
cro:substationDescription rdf:type owl:DatatypeProperty ;
                          rdfs:comment "A description of the substation and its components." ,
                                       "A detailed description of the substation, including its function, components, and significance within the electrical network." .


###  http://WSP.org/ontology/cro#substationInstallationDate
cro:substationInstallationDate rdf:type owl:DatatypeProperty ;
                               rdfs:comment "The date when the substation was installed." .


###  http://WSP.org/ontology/cro#substationLocatedIn
cro:substationLocatedIn rdf:type owl:DatatypeProperty ;
                        rdfs:comment "The specific location or site where the substation is situated, typically within the context of a larger facility or operational area." .


###  http://WSP.org/ontology/cro#substationName
cro:substationName rdf:type owl:DatatypeProperty ;
                   rdfs:comment "The name assigned to the substation." .


###  http://WSP.org/ontology/cro#summaryText
cro:summaryText rdf:type owl:DatatypeProperty ;
                rdfs:comment "Contains the summary of a recommendation." .


###  http://WSP.org/ontology/cro#supportNetwork
cro:supportNetwork rdf:type owl:DatatypeProperty ;
                   rdfs:comment "Indicates if the network supports other networks." ,
                                "The auxiliary or backup network that supports the primary electrical infrastructure, providing redundancy and additional capacity when needed." .


###  http://WSP.org/ontology/cro#suspendedRecommendationNumber
cro:suspendedRecommendationNumber rdf:type owl:DatatypeProperty .


###  http://WSP.org/ontology/cro#systemChangeDescription
cro:systemChangeDescription rdf:type owl:DatatypeProperty ;
                            rdfs:comment "A detailed description of the changes made to the systems within the operation, such as software updates or new system integrations." .


###  http://WSP.org/ontology/cro#systemChangeName
cro:systemChangeName rdf:type owl:DatatypeProperty ;
                     rdfs:comment "The name or title given to a specific system change or upgrade." .


###  http://WSP.org/ontology/cro#terminalName
cro:terminalName rdf:type owl:DatatypeProperty ;
                 rdfs:comment "The name of the terminal within the port, distinguishing it from other terminals." .


###  http://WSP.org/ontology/cro#timeSinceLastIncident
cro:timeSinceLastIncident rdf:type owl:DatatypeProperty ;
                          rdfs:comment "The amount of time that has passed since the last significant incident occurred." .


###  http://WSP.org/ontology/cro#tornado
cro:tornado rdf:type owl:DatatypeProperty ;
            rdfs:comment "Indicates the tornado risk or history for a specific location, used in environmental and risk assessments." .


###  http://WSP.org/ontology/cro#totalElectricityDemand
cro:totalElectricityDemand rdf:type owl:DatatypeProperty ;
                           rdfs:comment "The overall electricity demand that the Project aims to support, accounting for both current and future infrastructure needs." ,
                                        "The total electricity demand on the network." .


###  http://WSP.org/ontology/cro#totalLossUSDM
cro:totalLossUSDM rdf:type owl:DatatypeProperty .


###  http://WSP.org/ontology/cro#totalRecommendationNumber
cro:totalRecommendationNumber rdf:type owl:DatatypeProperty ;
                              rdfs:comment "Represents the total number of recommendations." .


###  http://WSP.org/ontology/cro#townName
cro:townName rdf:type owl:DatatypeProperty ;
             rdfs:comment "Name of the town" .


###  http://WSP.org/ontology/cro#transmissionLineType
cro:transmissionLineType rdf:type owl:DatatypeProperty ;
                         rdfs:comment "The type of transmission line, such as overhead or underground, and its voltage level, important for understanding its capacity and role in the network." .


###  http://WSP.org/ontology/cro#tropicalCyclone
cro:tropicalCyclone rdf:type owl:DatatypeProperty ;
                    rdfs:comment "Indicates the tropical cyclone risk or history for a specific location, used in environmental and risk assessments." .


###  http://WSP.org/ontology/cro#underReviewRecommendationNumber
cro:underReviewRecommendationNumber rdf:type owl:DatatypeProperty ;
                                    rdfs:comment "Represents the number of recommendations under review." .


###  http://WSP.org/ontology/cro#upgradeYear
cro:upgradeYear rdf:type owl:DatatypeProperty ;
                rdfs:comment "The year when a network component was last upgraded." .


###  http://WSP.org/ontology/cro#upgradedBy
cro:upgradedBy rdf:type owl:DatatypeProperty ;
               rdfs:comment "The entity or person responsible for upgrading the component." .


###  http://WSP.org/ontology/cro#utilityOrSupplyDescription
cro:utilityOrSupplyDescription rdf:type owl:DatatypeProperty ;
                               rdfs:comment "Any utilities of supplies that the site or operation depend on, such as water, electrocoty, gas, etc." .


###  http://WSP.org/ontology/cro#utilityOrSupplyName
cro:utilityOrSupplyName rdf:type owl:DatatypeProperty ;
                        rdfs:comment "Description of any utilities of supplies that the site or operation depend on, such as water, electrocoty, gas, etc" .


###  http://WSP.org/ontology/cro#ventilationAirflow
cro:ventilationAirflow rdf:type owl:DatatypeProperty .


###  http://WSP.org/ontology/cro#voltageLevel
cro:voltageLevel rdf:type owl:DatatypeProperty ;
                 rdfs:comment "The voltage level of the transmission line or substation." .


###  http://WSP.org/ontology/cro#wasteRockDumpHeight
cro:wasteRockDumpHeight rdf:type owl:DatatypeProperty .


###  http://WSP.org/ontology/cro#workCommencedBoolean
cro:workCommencedBoolean rdf:type owl:DatatypeProperty ;
                         rdfs:comment "Specify whether the project work has started or not." .


###  http://WSP.org/ontology/cro#workaround
cro:workaround rdf:type owl:DatatypeProperty ;
               rdfs:comment "Describes the workaround for handling an incident." .


#################################################################
#    Classes
#################################################################

###  http://WSP.org/ontology/cro#AssumptionsAndBasis
cro:AssumptionsAndBasis rdf:type owl:Class ;
                        rdfs:subClassOf [ rdf:type owl:Restriction ;
                                          owl:onProperty cro:assumptionDescription ;
                                          owl:someValuesFrom xsd:string
                                        ] ;
                        rdfs:comment "Class representing assumptions and basis for risk analysis." .


###  http://WSP.org/ontology/cro#AuditsAndReviews
cro:AuditsAndReviews rdf:type owl:Class ;
                     rdfs:subClassOf [ rdf:type owl:Restriction ;
                                       owl:onProperty cro:auditAndReviewDescription ;
                                       owl:someValuesFrom xsd:string
                                     ] ,
                                     [ rdf:type owl:Restriction ;
                                       owl:onProperty cro:auditReviewName ;
                                       owl:someValuesFrom xsd:string
                                     ] ;
                     rdfs:comment "Information on audits, compliance reviews, and assessments conducted since the last Critical Risk Assessment." .


###  http://WSP.org/ontology/cro#Berthing
cro:Berthing rdf:type owl:Class ;
             rdfs:subClassOf [ rdf:type owl:Restriction ;
                               owl:onProperty cro:hasEquipment ;
                               owl:someValuesFrom cro:Equipment
                             ] ,
                             [ rdf:type owl:Restriction ;
                               owl:onProperty cro:berthName ;
                               owl:someValuesFrom xsd:string
                             ] ,
                             [ rdf:type owl:Restriction ;
                               owl:onProperty cro:berthTerminal ;
                               owl:someValuesFrom xsd:string
                             ] ,
                             [ rdf:type owl:Restriction ;
                               owl:onProperty cro:dredgeDepth ;
                               owl:someValuesFrom xsd:decimal
                             ] ;
             rdfs:comment "Berthing refers to the process of securing vessels at a Port's docking facilities. This operation is crucial for the safe inloading and outloading of materials and involves the use of specialized Equipment." .


###  http://WSP.org/ontology/cro#CatastrophicRiskScenariosWithLowProbabilityOverview
cro:CatastrophicRiskScenariosWithLowProbabilityOverview rdf:type owl:Class ;
                                                        rdfs:subClassOf [ rdf:type owl:Restriction ;
                                                                          owl:onProperty cro:catastrophicRiskScenariowithLowProbability ;
                                                                          owl:someValuesFrom xsd:string
                                                                        ] ;
                                                        rdfs:comment "The definition of a catastrophic risk scenario with low probability as stated by the CRA Report: Risk scenarios beyond the boundaries of reasonable probability are infinite as to their potential diversity and application. Hence, scenarios with an occurrence probability beyond the 100 years return period cut- off point in the Critical Risk Assessment model have been excluded." .


###  http://WSP.org/ontology/cro#ChangeToRawMaterialsAndSales
cro:ChangeToRawMaterialsAndSales rdf:type owl:Class ;
                                 rdfs:subClassOf cro:SignificantChanges ,
                                                 [ rdf:type owl:Restriction ;
                                                   owl:onProperty cro:changeInProduction ;
                                                   owl:someValuesFrom xsd:string
                                                 ] ,
                                                 [ rdf:type owl:Restriction ;
                                                   owl:onProperty cro:changeInRawMaterial ;
                                                   owl:someValuesFrom xsd:string
                                                 ] ,
                                                 [ rdf:type owl:Restriction ;
                                                   owl:onProperty cro:changeInSales ;
                                                   owl:someValuesFrom xsd:string
                                                 ] ;
                                 rdfs:comment "Updates regarding production volumes, sales forecasts, and changes in raw materials handling since the last assessment." .


###  http://WSP.org/ontology/cro#ChangesToCriticalRiskScenarios
cro:ChangesToCriticalRiskScenarios rdf:type owl:Class ;
                                   rdfs:subClassOf cro:SignificantChanges ,
                                                   [ rdf:type owl:Restriction ;
                                                     owl:onProperty cro:changeInBusinessInterruption ;
                                                     owl:someValuesFrom xsd:string
                                                   ] ,
                                                   [ rdf:type owl:Restriction ;
                                                     owl:onProperty cro:changeInPortDescription ;
                                                     owl:someValuesFrom xsd:string
                                                   ] ,
                                                   [ rdf:type owl:Restriction ;
                                                     owl:onProperty cro:criticalRiskScenarioChangeFromPrevious ;
                                                     owl:someValuesFrom xsd:string
                                                   ] ,
                                                   [ rdf:type owl:Restriction ;
                                                     owl:onProperty cro:criticalRiskScenarioID ;
                                                     owl:someValuesFrom xsd:string
                                                   ] ;
                                   rdfs:comment "Modifications or updates to the critical risk scenarios and business interruption based on new data or operational changes." .


###  http://WSP.org/ontology/cro#ChangesToEquipmentAndFacilities
cro:ChangesToEquipmentAndFacilities rdf:type owl:Class ;
                                    rdfs:subClassOf cro:SignificantChanges ,
                                                    [ rdf:type owl:Restriction ;
                                                      owl:onProperty cro:equipmentChangeDescription ;
                                                      owl:someValuesFrom xsd:string
                                                    ] ,
                                                    [ rdf:type owl:Restriction ;
                                                      owl:onProperty cro:equipmentChanged ;
                                                      owl:someValuesFrom xsd:string
                                                    ] ,
                                                    [ rdf:type owl:Restriction ;
                                                      owl:onProperty cro:facilityChangeDescription ;
                                                      owl:someValuesFrom xsd:string
                                                    ] ,
                                                    [ rdf:type owl:Restriction ;
                                                      owl:onProperty cro:facilityChanged ;
                                                      owl:someValuesFrom xsd:string
                                                    ] ;
                                    rdfs:comment "Details of upgrades, repairs, and significant works on equipment and facilities that have occurred or are planned." .


###  http://WSP.org/ontology/cro#Company
cro:Company rdf:type owl:Class ;
            rdfs:subClassOf [ rdf:type owl:Restriction ;
                              owl:onProperty cro:hasDivision ;
                              owl:someValuesFrom cro:Division
                            ] ,
                            [ rdf:type owl:Restriction ;
                              owl:onProperty cro:hasEmployee ;
                              owl:someValuesFrom cro:Employee
                            ] ,
                            [ rdf:type owl:Restriction ;
                              owl:onProperty cro:hasBusiness ;
                              owl:someValuesFrom xsd:string
                            ] ,
                            [ rdf:type owl:Restriction ;
                              owl:onProperty cro:hasCompanyName ;
                              owl:someValuesFrom xsd:string
                            ] ;
            rdfs:comment "Company refers to the entity that owns or participates in the operation, including owners, consultants, and other stakeholders. Companies can have divisions responsible for different aspects of the operation. They also manage CRAs (Critical Risk Assessments) and related data." .


###  http://WSP.org/ontology/cro#Contacts
cro:Contacts rdf:type owl:Class ;
             rdfs:subClassOf cro:SurveyAndReportDetails ,
                             [ rdf:type owl:Restriction ;
                               owl:onProperty cro:contactName ;
                               owl:someValuesFrom xsd:string
                             ] ,
                             [ rdf:type owl:Restriction ;
                               owl:onProperty cro:contactRole ;
                               owl:someValuesFrom xsd:string
                             ] ;
             rdfs:comment "Class representing contact information." .


###  http://WSP.org/ontology/cro#CriticalRiskAssesmentReport
cro:CriticalRiskAssesmentReport rdf:type owl:Class ;
                                rdfs:subClassOf [ rdf:type owl:Restriction ;
                                                  owl:onProperty cro:distributedTo ;
                                                  owl:someValuesFrom cro:Employee
                                                ] ,
                                                [ rdf:type owl:Restriction ;
                                                  owl:onProperty cro:hasAuditsAndReviews ;
                                                  owl:someValuesFrom cro:AuditsAndReviews
                                                ] ,
                                                [ rdf:type owl:Restriction ;
                                                  owl:onProperty cro:hasCriticalRiskScenarioOverview ;
                                                  owl:someValuesFrom cro:CriticalRiskSectionOverview
                                                ] ,
                                                [ rdf:type owl:Restriction ;
                                                  owl:onProperty cro:hasIdentifiedRecommendations ;
                                                  owl:someValuesFrom cro:Recommendation
                                                ] ,
                                                [ rdf:type owl:Restriction ;
                                                  owl:onProperty cro:hasRevision ;
                                                  owl:someValuesFrom cro:Revision
                                                ] ,
                                                [ rdf:type owl:Restriction ;
                                                  owl:onProperty cro:hasRiskManagementSystem ;
                                                  owl:someValuesFrom cro:RiskManagementSystem
                                                ] ,
                                                [ rdf:type owl:Restriction ;
                                                  owl:onProperty cro:hasSignificantChanges ;
                                                  owl:someValuesFrom cro:SignificantChanges
                                                ] ,
                                                [ rdf:type owl:Restriction ;
                                                  owl:onProperty cro:hasSignificantIncidents ;
                                                  owl:someValuesFrom cro:SignificantIncident
                                                ] ,
                                                [ rdf:type owl:Restriction ;
                                                  owl:onProperty cro:hasSurveyAndReportDetails ;
                                                  owl:someValuesFrom cro:SurveyAndReportDetails
                                                ] ,
                                                [ rdf:type owl:Restriction ;
                                                  owl:onProperty cro:preparedBy ;
                                                  owl:someValuesFrom cro:Employee
                                                ] ,
                                                [ rdf:type owl:Restriction ;
                                                  owl:onProperty cro:currentSurveyRatingSummaryPercentage ;
                                                  owl:someValuesFrom xsd:int
                                                ] ,
                                                [ rdf:type owl:Restriction ;
                                                  owl:onProperty cro:hasCRADate ;
                                                  owl:someValuesFrom xsd:dateTime
                                                ] ,
                                                [ rdf:type owl:Restriction ;
                                                  owl:onProperty cro:hasCRAType ;
                                                  owl:someValuesFrom xsd:string
                                                ] ,
                                                [ rdf:type owl:Restriction ;
                                                  owl:onProperty cro:hasDateOfSurvey ;
                                                  owl:someValuesFrom xsd:dateTime
                                                ] ,
                                                [ rdf:type owl:Restriction ;
                                                  owl:onProperty cro:previousSurveyRatingSummaryPercentage ;
                                                  owl:someValuesFrom xsd:int
                                                ] ;
                                rdfs:comment "CRA (Critical Risk Assessment) refers to a comprehensive evaluation conducted to identify and mitigate risks associated with operations. It typically includes detailed analysis using NATHAN Data and is prepared, revised, and distributed by employees to ensure operational safety and compliance." .


###  http://WSP.org/ontology/cro#CriticalRiskScenario
cro:CriticalRiskScenario rdf:type owl:Class ;
                         rdfs:subClassOf [ rdf:type owl:Restriction ;
                                           owl:onProperty cro:hasRecommendation ;
                                           owl:someValuesFrom cro:Recommendation
                                         ] ,
                                         [ rdf:type owl:Restriction ;
                                           owl:onProperty cro:impactsOperation ;
                                           owl:someValuesFrom cro:Operation
                                         ] ,
                                         [ rdf:type owl:Restriction ;
                                           owl:onProperty cro:riskImpactsEquipment ;
                                           owl:someValuesFrom cro:Equipment
                                         ] ,
                                         [ rdf:type owl:Restriction ;
                                           owl:onProperty cro:riskImpactsFacility ;
                                           owl:someValuesFrom cro:Facility
                                         ] ,
                                         [ rdf:type owl:Restriction ;
                                           owl:onProperty cro:BISummary ;
                                           owl:someValuesFrom xsd:string
                                         ] ,
                                         [ rdf:type owl:Restriction ;
                                           owl:onProperty cro:assetGroup ;
                                           owl:someValuesFrom xsd:string
                                         ] ,
                                         [ rdf:type owl:Restriction ;
                                           owl:onProperty cro:businessInterruptionUSDM ;
                                           owl:someValuesFrom xsd:decimal
                                         ] ,
                                         [ rdf:type owl:Restriction ;
                                           owl:onProperty cro:criticalRiskScenarioID ;
                                           owl:someValuesFrom xsd:string
                                         ] ,
                                         [ rdf:type owl:Restriction ;
                                           owl:onProperty cro:hardControls ;
                                           owl:someValuesFrom xsd:string
                                         ] ,
                                         [ rdf:type owl:Restriction ;
                                           owl:onProperty cro:incidentDescription ;
                                           owl:someValuesFrom xsd:string
                                         ] ,
                                         [ rdf:type owl:Restriction ;
                                           owl:onProperty cro:incidentSummary ;
                                           owl:someValuesFrom xsd:string
                                         ] ,
                                         [ rdf:type owl:Restriction ;
                                           owl:onProperty cro:inherentControls ;
                                           owl:someValuesFrom xsd:string
                                         ] ,
                                         [ rdf:type owl:Restriction ;
                                           owl:onProperty cro:inherentHazards ;
                                           owl:someValuesFrom xsd:string
                                         ] ,
                                         [ rdf:type owl:Restriction ;
                                           owl:onProperty cro:likelihood ;
                                           owl:someValuesFrom xsd:string
                                         ] ,
                                         [ rdf:type owl:Restriction ;
                                           owl:onProperty cro:lossScenarioPeril ;
                                           owl:someValuesFrom xsd:string
                                         ] ,
                                         [ rdf:type owl:Restriction ;
                                           owl:onProperty cro:otherCostsUSDM ;
                                           owl:someValuesFrom xsd:decimal
                                         ] ,
                                         [ rdf:type owl:Restriction ;
                                           owl:onProperty cro:preincident_and_workaroundARP ;
                                           owl:someValuesFrom xsd:string
                                         ] ,
                                         [ rdf:type owl:Restriction ;
                                           owl:onProperty cro:propertyDamageUSDM ;
                                           owl:someValuesFrom xsd:decimal
                                         ] ,
                                         [ rdf:type owl:Restriction ;
                                           owl:onProperty cro:recommendationDescription ;
                                           owl:someValuesFrom xsd:string
                                         ] ,
                                         [ rdf:type owl:Restriction ;
                                           owl:onProperty cro:recoveryRepair ;
                                           owl:someValuesFrom xsd:string
                                         ] ,
                                         [ rdf:type owl:Restriction ;
                                           owl:onProperty cro:repairPeriod ;
                                           owl:someValuesFrom xsd:string
                                         ] ,
                                         [ rdf:type owl:Restriction ;
                                           owl:onProperty cro:softControls ;
                                           owl:someValuesFrom xsd:string
                                         ] ,
                                         [ rdf:type owl:Restriction ;
                                           owl:onProperty cro:totalLossUSDM ;
                                           owl:someValuesFrom xsd:decimal
                                         ] ,
                                         [ rdf:type owl:Restriction ;
                                           owl:onProperty cro:workaround ;
                                           owl:someValuesFrom xsd:string
                                         ] ;
                         rdfs:comment "Class representing critical risk scenarios." .


###  http://WSP.org/ontology/cro#CriticalRiskSectionOverview
cro:CriticalRiskSectionOverview rdf:type owl:Class ;
                                rdfs:subClassOf [ rdf:type owl:Restriction ;
                                                  owl:onProperty cro:hasAssumptions ;
                                                  owl:someValuesFrom cro:AssumptionsAndBasis
                                                ] ,
                                                [ rdf:type owl:Restriction ;
                                                  owl:onProperty cro:hasCatastrophicRiskScenariosWithLowProbability ;
                                                  owl:someValuesFrom cro:CatastrophicRiskScenariosWithLowProbabilityOverview
                                                ] ,
                                                [ rdf:type owl:Restriction ;
                                                  owl:onProperty cro:hasDependencies ;
                                                  owl:someValuesFrom cro:Dependencies
                                                ] ,
                                                [ rdf:type owl:Restriction ;
                                                  owl:onProperty cro:criticaRiskScenarioDefinition ;
                                                  owl:someValuesFrom xsd:string
                                                ] ,
                                                [ rdf:type owl:Restriction ;
                                                  owl:onProperty cro:generalInformationDescription ;
                                                  owl:someValuesFrom xsd:string
                                                ] ,
                                                [ rdf:type owl:Restriction ;
                                                  owl:onProperty cro:riskLikelihoodClassification ;
                                                  owl:someValuesFrom xsd:string
                                                ] ;
                                rdfs:comment "Class representing an overview of critical risk scenarios." .


###  http://WSP.org/ontology/cro#Dependencies
cro:Dependencies rdf:type owl:Class ;
                 rdfs:subClassOf [ rdf:type owl:Restriction ;
                                   owl:onProperty cro:dependencyDefinition ;
                                   owl:someValuesFrom xsd:string
                                 ] ;
                 rdfs:comment "Class representing dependencies in risk scenarios." .


###  http://WSP.org/ontology/cro#DieselGenerator
cro:DieselGenerator rdf:type owl:Class ;
                    rdfs:subClassOf [ rdf:type owl:Restriction ;
                                      owl:onProperty cro:generatorCapacity ;
                                      owl:someValuesFrom xsd:decimal
                                    ] ;
                    rdfs:comment "A generator that runs on diesel fuel." .


###  http://WSP.org/ontology/cro#DistributionSystem
cro:DistributionSystem rdf:type owl:Class ;
                       rdfs:subClassOf [ rdf:type owl:Restriction ;
                                         owl:onProperty cro:hasSubstation ;
                                         owl:someValuesFrom cro:Substation
                                       ] ,
                                       [ rdf:type owl:Restriction ;
                                         owl:onProperty cro:hasTransmissionLine ;
                                         owl:someValuesFrom cro:TransmissionLine
                                       ] ,
                                       [ rdf:type owl:Restriction ;
                                         owl:onProperty cro:distributionSystemDescription ;
                                         owl:someValuesFrom xsd:string
                                       ] ,
                                       [ rdf:type owl:Restriction ;
                                         owl:onProperty cro:distributionSystemName ;
                                         owl:someValuesFrom xsd:string
                                       ] ;
                       rdfs:comment "A system for distributing electricity from power stations to end users." .


###  http://WSP.org/ontology/cro#Division
cro:Division rdf:type owl:Class ;
             rdfs:subClassOf [ rdf:type owl:Restriction ;
                               owl:onProperty cro:divisionDescription ;
                               owl:someValuesFrom xsd:string
                             ] ;
             rdfs:comment "Division refers to a subset of a Company responsible for specific aspects of an Operation. Divisions may focus on areas such as safety, production, or logistics within the broader operation." .


###  http://WSP.org/ontology/cro#Embankment
cro:Embankment rdf:type owl:Class ;
               rdfs:subClassOf [ rdf:type owl:Restriction ;
                                 owl:onProperty cro:constructionMethod ;
                                 owl:someValuesFrom xsd:string
                               ] ,
                               [ rdf:type owl:Restriction ;
                                 owl:onProperty cro:embankmentHeight ;
                                 owl:someValuesFrom xsd:decimal
                               ] ,
                               [ rdf:type owl:Restriction ;
                                 owl:onProperty cro:embankmentLength ;
                                 owl:someValuesFrom xsd:decimal
                               ] .


###  http://WSP.org/ontology/cro#Employee
cro:Employee rdf:type owl:Class ;
             rdfs:subClassOf [ rdf:type owl:Restriction ;
                               owl:onProperty cro:hasEmployeeEmail ;
                               owl:someValuesFrom xsd:string
                             ] ,
                             [ rdf:type owl:Restriction ;
                               owl:onProperty cro:hasEmployeePhoneNumber ;
                               owl:someValuesFrom xsd:string
                             ] ,
                             [ rdf:type owl:Restriction ;
                               owl:onProperty cro:hasFirstName ;
                               owl:someValuesFrom xsd:string
                             ] ,
                             [ rdf:type owl:Restriction ;
                               owl:onProperty cro:hasLastName ;
                               owl:someValuesFrom xsd:string
                             ] ;
             rdfs:comment "Employee refers to individuals who work for a Company, contributing to the Operation in various capacities. Employees may be involved in preparing, distributing, and revising CRAs and other critical documentation." .


###  http://WSP.org/ontology/cro#EngineerOfRecord
cro:EngineerOfRecord rdf:type owl:Class ;
                     rdfs:subClassOf cro:Employee ,
                                     [ rdf:type owl:Restriction ;
                                       owl:onProperty cro:responsibleFor ;
                                       owl:someValuesFrom cro:TailingsStorageFacility
                                     ] ,
                                     [ rdf:type owl:Restriction ;
                                       owl:onProperty cro:appointmentDate ;
                                       owl:someValuesFrom xsd:string
                                     ] .


###  http://WSP.org/ontology/cro#Equipment
cro:Equipment rdf:type owl:Class ;
              rdfs:subClassOf [ rdf:type owl:Restriction ;
                                owl:onProperty cro:agedConditionBoolean ;
                                owl:someValuesFrom xsd:boolean
                              ] ,
                              [ rdf:type owl:Restriction ;
                                owl:onProperty cro:amountOfEquipmentAvailable ;
                                owl:someValuesFrom xsd:int
                              ] ,
                              [ rdf:type owl:Restriction ;
                                owl:onProperty cro:equipmentDescription ;
                                owl:someValuesFrom xsd:string
                              ] ,
                              [ rdf:type owl:Restriction ;
                                owl:onProperty cro:equipmentName ;
                                owl:someValuesFrom xsd:string
                              ] ,
                              [ rdf:type owl:Restriction ;
                                owl:onProperty cro:equipmentReplacedDate ;
                                owl:someValuesFrom xsd:dateTime
                              ] ,
                              [ rdf:type owl:Restriction ;
                                owl:onProperty cro:equipmentType ;
                                owl:someValuesFrom xsd:string
                              ] ;
              rdfs:comment "Equipment refers to the tools, machinery, and resources used in various operations, including mining, port activities, and marine operations. Equipment is associated with specific Facilities and Processes within the operation." .


###  http://WSP.org/ontology/cro#ExternalEnvironmentChanges
cro:ExternalEnvironmentChanges rdf:type owl:Class ;
                               rdfs:subClassOf cro:SignificantChanges ,
                                               [ rdf:type owl:Restriction ;
                                                 owl:onProperty cro:changeInEnvironment ;
                                                 owl:someValuesFrom xsd:string
                                               ] ,
                                               [ rdf:type owl:Restriction ;
                                                 owl:onProperty cro:changeInEnvironmentDescription ;
                                                 owl:someValuesFrom xsd:string
                                               ] ;
                               rdfs:comment "Information on changes in external factors, such as environmental conditions or market dynamics, that impact operations." .


###  http://WSP.org/ontology/cro#Facility
cro:Facility rdf:type owl:Class ;
             rdfs:subClassOf [ rdf:type owl:Restriction ;
                               owl:onProperty cro:hasEquipment ;
                               owl:someValuesFrom cro:Equipment
                             ] ,
                             [ rdf:type owl:Restriction ;
                               owl:onProperty cro:hasProcess ;
                               owl:someValuesFrom cro:FacilityProcess
                             ] ,
                             [ rdf:type owl:Restriction ;
                               owl:onProperty cro:facilityDescription ;
                               owl:someValuesFrom xsd:string
                             ] ,
                             [ rdf:type owl:Restriction ;
                               owl:onProperty cro:facilityName ;
                               owl:someValuesFrom xsd:string
                             ] ;
             rdfs:comment """These Asset Groups are: 
• Mining (includes tailings dam) 
• Treatment (milling, concentrating, conditioning) 
• Smelting 
• Refining 
• Materials Handling 
• Transport (ship, rail, road, product pipeline, air) 
• Power Distribution 
• Power Generation 
• Water Supply 
• Port Facilities""" .


###  http://WSP.org/ontology/cro#FacilityProcess
cro:FacilityProcess rdf:type owl:Class ;
                    rdfs:subClassOf [ rdf:type owl:Restriction ;
                                      owl:onProperty cro:processDescription ;
                                      owl:someValuesFrom xsd:string
                                    ] ;
                    rdfs:comment "Facility Process refers to specific activities or workflows carried out within a Facility. These processes are essential for maintaining the operation of the Facility and may involve the use of specialized Equipment." .


###  http://WSP.org/ontology/cro#FinalProduct
cro:FinalProduct rdf:type owl:Class ;
                 rdfs:subClassOf cro:Dependencies ,
                                 [ rdf:type owl:Restriction ;
                                   owl:onProperty cro:finalProductDescription ;
                                   owl:someValuesFrom xsd:string
                                 ] ;
                 rdfs:comment "Class representing final product details." .


###  http://WSP.org/ontology/cro#Inloading
cro:Inloading rdf:type owl:Class ;
              rdfs:subClassOf [ rdf:type owl:Restriction ;
                                owl:onProperty cro:hasEquipment ;
                                owl:someValuesFrom cro:Equipment
                              ] ,
                              [ rdf:type owl:Restriction ;
                                owl:onProperty cro:hasProcess ;
                                owl:someValuesFrom cro:FacilityProcess
                              ] ,
                              [ rdf:type owl:Restriction ;
                                owl:onProperty cro:inloadingDescription ;
                                owl:someValuesFrom xsd:string
                              ] ,
                              [ rdf:type owl:Restriction ;
                                owl:onProperty cro:inloadsMaterialFrom ;
                                owl:someValuesFrom xsd:string
                              ] ;
              rdfs:comment "Inloading refers to the marine operation involving the receipt and handling of materials or goods at a Port Facility. This process includes the use of Equipment such as cranes, conveyors, and vessels." .


###  http://WSP.org/ontology/cro#MFL_Report
cro:MFL_Report rdf:type owl:Class ;
               rdfs:subClassOf cro:CriticalRiskAssesmentReport ,
                               [ rdf:type owl:Restriction ;
                                 owl:onProperty cro:hasIdentifiedCriticalRiskScenarios ;
                                 owl:someValuesFrom cro:CriticalRiskScenario
                               ] .


###  http://WSP.org/ontology/cro#MaterialHandling
cro:MaterialHandling rdf:type owl:Class ;
                     rdfs:subClassOf cro:Facility .


###  http://WSP.org/ontology/cro#Materials
cro:Materials rdf:type owl:Class ;
              rdfs:subClassOf cro:Dependencies ,
                              [ rdf:type owl:Restriction ;
                                owl:onProperty cro:rawMaterialDescription ;
                                owl:someValuesFrom xsd:string
                              ] ,
                              [ rdf:type owl:Restriction ;
                                owl:onProperty cro:rawMaterialName ;
                                owl:someValuesFrom xsd:string
                              ] ;
              rdfs:comment "Class representing materials in the report." .


###  http://WSP.org/ontology/cro#Mine
cro:Mine rdf:type owl:Class ;
         rdfs:subClassOf cro:Operation ,
                         [ rdf:type owl:Restriction ;
                           owl:onProperty cro:hasTSF ;
                           owl:someValuesFrom cro:TailingsStorageFacility
                         ] ,
                         [ rdf:type owl:Restriction ;
                           owl:onProperty cro:designDate ;
                           owl:someValuesFrom xsd:string
                         ] ,
                         [ rdf:type owl:Restriction ;
                           owl:onProperty cro:mineLocation ;
                           owl:someValuesFrom xsd:string
                         ] ,
                         [ rdf:type owl:Restriction ;
                           owl:onProperty cro:mineName ;
                           owl:someValuesFrom xsd:string
                         ] ,
                         [ rdf:type owl:Restriction ;
                           owl:onProperty cro:mineType ;
                           owl:someValuesFrom xsd:string
                         ] .


###  http://WSP.org/ontology/cro#NATHANData
cro:NATHANData rdf:type owl:Class ;
               rdfs:subClassOf [ rdf:type owl:Restriction ;
                                 owl:onProperty cro:Tsunami ;
                                 owl:someValuesFrom xsd:string
                               ] ,
                               [ rdf:type owl:Restriction ;
                                 owl:onProperty cro:earthquakeZone ;
                                 owl:someValuesFrom xsd:string
                               ] ,
                               [ rdf:type owl:Restriction ;
                                 owl:onProperty cro:extratropicalCycloner ;
                                 owl:someValuesFrom xsd:string
                               ] ,
                               [ rdf:type owl:Restriction ;
                                 owl:onProperty cro:flood ;
                                 owl:someValuesFrom xsd:string
                               ] ,
                               [ rdf:type owl:Restriction ;
                                 owl:onProperty cro:stormSurge ;
                                 owl:someValuesFrom xsd:string
                               ] ,
                               [ rdf:type owl:Restriction ;
                                 owl:onProperty cro:tornado ;
                                 owl:someValuesFrom xsd:string
                               ] ,
                               [ rdf:type owl:Restriction ;
                                 owl:onProperty cro:tropicalCyclone ;
                                 owl:someValuesFrom xsd:string
                               ] ;
               rdfs:comment "NATHAN Data refers to specific information used in Critical Risk Assessments (CRAs) to assess and mitigate risks in operations. This data is prepared by Employees, distributed, and revised within a Company." .


###  http://WSP.org/ontology/cro#NLE_Report
cro:NLE_Report rdf:type owl:Class ;
               rdfs:subClassOf cro:CriticalRiskAssesmentReport ,
                               [ rdf:type owl:Restriction ;
                                 owl:onProperty cro:hasIdentifiedCriticalRiskScenarios ;
                                 owl:someValuesFrom cro:CriticalRiskScenario
                               ] .


###  http://WSP.org/ontology/cro#OpenPit
cro:OpenPit rdf:type owl:Class ;
            rdfs:subClassOf cro:Mine ,
                            [ rdf:type owl:Restriction ;
                              owl:onProperty cro:benchHeight ;
                              owl:someValuesFrom xsd:decimal
                            ] ,
                            [ rdf:type owl:Restriction ;
                              owl:onProperty cro:bermWidth ;
                              owl:someValuesFrom xsd:decimal
                            ] ,
                            [ rdf:type owl:Restriction ;
                              owl:onProperty cro:slopeAngle ;
                              owl:someValuesFrom xsd:string
                            ] ,
                            [ rdf:type owl:Restriction ;
                              owl:onProperty cro:stockpileCapacity ;
                              owl:someValuesFrom xsd:decimal
                            ] ,
                            [ rdf:type owl:Restriction ;
                              owl:onProperty cro:wasteRockDumpHeight ;
                              owl:someValuesFrom xsd:decimal
                            ] .


###  http://WSP.org/ontology/cro#Operation
cro:Operation rdf:type owl:Class ;
              rdfs:subClassOf [ rdf:type owl:Restriction ;
                                owl:onProperty cro:hasFacility ;
                                owl:someValuesFrom cro:Facility
                              ] ,
                              [ rdf:type owl:Restriction ;
                                owl:onProperty cro:hasProcessControl ;
                                owl:someValuesFrom cro:ProcessControlAutomationSystem
                              ] ,
                              [ rdf:type owl:Restriction ;
                                owl:onProperty cro:hasProject ;
                                owl:someValuesFrom cro:Project
                              ] ,
                              [ rdf:type owl:Restriction ;
                                owl:onProperty cro:hasRiskAssessmentReport ;
                                owl:someValuesFrom cro:CriticalRiskAssesmentReport
                              ] ,
                              [ rdf:type owl:Restriction ;
                                owl:onProperty cro:operatedBy ;
                                owl:someValuesFrom cro:Division
                              ] ,
                              [ rdf:type owl:Restriction ;
                                owl:onProperty cro:ownedBy ;
                                owl:someValuesFrom cro:Company
                              ] ,
                              [ rdf:type owl:Restriction ;
                                owl:onProperty <http://WSP.org/ontology/cro/hasMFLRiskAssessmentReports> ;
                                owl:someValuesFrom cro:MFL_Report
                              ] ,
                              [ rdf:type owl:Restriction ;
                                owl:onProperty <http://WSP.org/ontology/cro/hasNLERiskAssessmentReports> ;
                                owl:someValuesFrom cro:NLE_Report
                              ] ,
                              [ rdf:type owl:Restriction ;
                                owl:onProperty cro:electricityDemand ;
                                owl:someValuesFrom xsd:decimal
                              ] ,
                              [ rdf:type owl:Restriction ;
                                owl:onProperty cro:hasAddress ;
                                owl:someValuesFrom xsd:string
                              ] ,
                              [ rdf:type owl:Restriction ;
                                owl:onProperty cro:hasEmail ;
                                owl:someValuesFrom xsd:string
                              ] ,
                              [ rdf:type owl:Restriction ;
                                owl:onProperty cro:hasLatitude ;
                                owl:someValuesFrom xsd:decimal
                              ] ,
                              [ rdf:type owl:Restriction ;
                                owl:onProperty cro:hasLongitude ;
                                owl:someValuesFrom xsd:decimal
                              ] ,
                              [ rdf:type owl:Restriction ;
                                owl:onProperty cro:hasName ;
                                owl:someValuesFrom xsd:string
                              ] ,
                              [ rdf:type owl:Restriction ;
                                owl:onProperty cro:hasPhone ;
                                owl:someValuesFrom xsd:string
                              ] ;
              rdfs:comment "Operation refers to the broader activity or process taking place in a specific location, such as mining, chemical processing, or port operations. The Operation class serves as a general category, with specific types of operations, such as Port or Smelting, being subclasses." .


###  http://WSP.org/ontology/cro#OreBody
cro:OreBody rdf:type owl:Class ;
            rdfs:subClassOf [ rdf:type owl:Restriction ;
                              owl:onProperty cro:containedIn ;
                              owl:someValuesFrom cro:Mine
                            ] ,
                            [ rdf:type owl:Restriction ;
                              owl:onProperty cro:providesOreForProcessing ;
                              owl:someValuesFrom cro:ProcessingPlant
                            ] ,
                            [ rdf:type owl:Restriction ;
                              owl:onProperty cro:grade ;
                              owl:someValuesFrom xsd:string
                            ] ,
                            [ rdf:type owl:Restriction ;
                              owl:onProperty cro:oreBodyName ;
                              owl:someValuesFrom xsd:string
                            ] .


###  http://WSP.org/ontology/cro#OrganisationalChanges
cro:OrganisationalChanges rdf:type owl:Class ;
                          rdfs:subClassOf cro:SignificantChanges ,
                                          [ rdf:type owl:Restriction ;
                                            owl:onProperty cro:organisationalChangeDescription ;
                                            owl:someValuesFrom xsd:string
                                          ] ;
                          rdfs:comment "Updates on changes within the organizational structure, including new appointments or shifts in management roles." .


###  http://WSP.org/ontology/cro#Other
cro:Other rdf:type owl:Class ;
          rdfs:subClassOf cro:Dependencies ,
                          [ rdf:type owl:Restriction ;
                            owl:onProperty cro:otherDependenciesDescription ;
                            owl:someValuesFrom xsd:string
                          ] ;
          rdfs:comment "Class representing any other dependencies or details." .


###  http://WSP.org/ontology/cro#Outloading
cro:Outloading rdf:type owl:Class ;
               rdfs:subClassOf [ rdf:type owl:Restriction ;
                                 owl:onProperty cro:hasEquipment ;
                                 owl:someValuesFrom cro:Equipment
                               ] ,
                               [ rdf:type owl:Restriction ;
                                 owl:onProperty cro:hasProcess ;
                                 owl:someValuesFrom cro:FacilityProcess
                               ] ,
                               [ rdf:type owl:Restriction ;
                                 owl:onProperty cro:outloadingDescription ;
                                 owl:someValuesFrom xsd:string
                               ] ,
                               [ rdf:type owl:Restriction ;
                                 owl:onProperty cro:outloadsMaterialTo ;
                                 owl:someValuesFrom xsd:string
                               ] ;
               rdfs:comment "Outloading refers to the marine operation involving the dispatch of materials or goods from a Port Facility. Similar to inloading, this process relies on Equipment and coordination within the Port." .


###  http://WSP.org/ontology/cro#Port
cro:Port rdf:type owl:Class ;
         rdfs:subClassOf cro:Operation ,
                         [ rdf:type owl:Restriction ;
                           owl:onProperty cro:hasMarineOperation ;
                           owl:someValuesFrom cro:Berthing
                         ] ,
                         [ rdf:type owl:Restriction ;
                           owl:onProperty cro:hasTerminal ;
                           owl:someValuesFrom cro:PortTerminal
                         ] ,
                         [ rdf:type owl:Restriction ;
                           owl:onProperty cro:numberOfContractors ;
                           owl:someValuesFrom xsd:int
                         ] ,
                         [ rdf:type owl:Restriction ;
                           owl:onProperty cro:numberOfEmployees ;
                           owl:someValuesFrom xsd:int
                         ] ,
                         [ rdf:type owl:Restriction ;
                           owl:onProperty cro:portName ;
                           owl:someValuesFrom xsd:string
                         ] ;
         rdfs:comment "Port refers to the operational area where marine activities, including inloading, outloading, and berthing, occur. The Port includes various Facilities, Terminals, and Equipment necessary for these operations." .


###  http://WSP.org/ontology/cro#PortTerminal
cro:PortTerminal rdf:type owl:Class ;
                 rdfs:subClassOf cro:Facility ,
                                 [ rdf:type owl:Restriction ;
                                   owl:onProperty cro:hasInloading ;
                                   owl:someValuesFrom cro:Inloading
                                 ] ,
                                 [ rdf:type owl:Restriction ;
                                   owl:onProperty cro:hasOutloading ;
                                   owl:someValuesFrom cro:Outloading
                                 ] ,
                                 [ rdf:type owl:Restriction ;
                                   owl:onProperty cro:ShipsMaterialTo ;
                                   owl:someValuesFrom xsd:string
                                 ] ,
                                 [ rdf:type owl:Restriction ;
                                   owl:onProperty cro:electricityDemand ;
                                   owl:someValuesFrom xsd:decimal
                                 ] ,
                                 [ rdf:type owl:Restriction ;
                                   owl:onProperty cro:materialHandled ;
                                   owl:someValuesFrom xsd:string
                                 ] ,
                                 [ rdf:type owl:Restriction ;
                                   owl:onProperty cro:materialHandledAmount ;
                                   owl:someValuesFrom xsd:decimal
                                 ] ,
                                 [ rdf:type owl:Restriction ;
                                   owl:onProperty cro:operationDescription ;
                                   owl:someValuesFrom xsd:string
                                 ] ,
                                 [ rdf:type owl:Restriction ;
                                   owl:onProperty cro:powerDemand ;
                                   owl:someValuesFrom xsd:decimal
                                 ] ,
                                 [ rdf:type owl:Restriction ;
                                   owl:onProperty cro:recievesMaterialFrom ;
                                   owl:someValuesFrom xsd:string
                                 ] ,
                                 [ rdf:type owl:Restriction ;
                                   owl:onProperty cro:terminalName ;
                                   owl:someValuesFrom xsd:string
                                 ] ;
                 rdfs:comment "Port Terminal refers to specific areas within a Port where goods or materials are loaded, unloaded, or stored. Terminals are integral to the operation of a Port and are equipped with the necessary infrastructure." .


###  http://WSP.org/ontology/cro#PowerStation
cro:PowerStation rdf:type owl:Class ;
                 rdfs:subClassOf cro:Facility ,
                                 [ rdf:type owl:Restriction ;
                                   owl:onProperty cro:hasDieselGenerator ;
                                   owl:someValuesFrom cro:DieselGenerator
                                 ] ,
                                 [ rdf:type owl:Restriction ;
                                   owl:onProperty cro:hasDistributionSystem ;
                                   owl:someValuesFrom cro:DistributionSystem
                                 ] ,
                                 [ rdf:type owl:Restriction ;
                                   owl:onProperty cro:hasPowerStation ;
                                   owl:someValuesFrom cro:PowerStation
                                 ] ,
                                 [ rdf:type owl:Restriction ;
                                   owl:onProperty cro:hasTurbine ;
                                   owl:someValuesFrom cro:Turbine
                                 ] ,
                                 [ rdf:type owl:Restriction ;
                                   owl:onProperty cro:operatedBy ;
                                   owl:someValuesFrom cro:Company
                                 ] ,
                                 [ rdf:type owl:Restriction ;
                                   owl:onProperty cro:ownedBy ;
                                   owl:someValuesFrom cro:Company
                                 ] ,
                                 [ rdf:type owl:Restriction ;
                                   owl:onProperty cro:suppliesPowerTo ;
                                   owl:someValuesFrom cro:Operation
                                 ] ,
                                 [ rdf:type owl:Restriction ;
                                   owl:onProperty cro:suppliesPowerTo ;
                                   owl:someValuesFrom cro:Town
                                 ] ,
                                 [ rdf:type owl:Restriction ;
                                   owl:onProperty cro:networkDescription ;
                                   owl:someValuesFrom xsd:string
                                 ] ,
                                 [ rdf:type owl:Restriction ;
                                   owl:onProperty cro:networkName ;
                                   owl:someValuesFrom xsd:string
                                 ] ,
                                 [ rdf:type owl:Restriction ;
                                   owl:onProperty cro:powerStationCapacity ;
                                   owl:someValuesFrom xsd:decimal
                                 ] ,
                                 [ rdf:type owl:Restriction ;
                                   owl:onProperty cro:powerStationDescription ;
                                   owl:someValuesFrom xsd:string
                                 ] ,
                                 [ rdf:type owl:Restriction ;
                                   owl:onProperty cro:powerStationLocation ;
                                   owl:someValuesFrom xsd:string
                                 ] ,
                                 [ rdf:type owl:Restriction ;
                                   owl:onProperty cro:powerStationName ;
                                   owl:someValuesFrom xsd:string
                                 ] ,
                                 [ rdf:type owl:Restriction ;
                                   owl:onProperty cro:powerStationType ;
                                   owl:someValuesFrom xsd:string
                                 ] ,
                                 [ rdf:type owl:Restriction ;
                                   owl:onProperty cro:region ;
                                   owl:someValuesFrom xsd:string
                                 ] ,
                                 [ rdf:type owl:Restriction ;
                                   owl:onProperty cro:supportNetwork ;
                                   owl:someValuesFrom xsd:string
                                 ] ,
                                 [ rdf:type owl:Restriction ;
                                   owl:onProperty cro:totalElectricityDemand ;
                                   owl:someValuesFrom xsd:decimal
                                 ] ;
                 rdfs:comment "A facility where electricity is generated, typically containing turbines and generators." ,
                              "A network responsible for generating and distributing electricity." .


###  http://WSP.org/ontology/cro#ProcessControlAutomationSystem
cro:ProcessControlAutomationSystem rdf:type owl:Class ;
                                   rdfs:subClassOf [ rdf:type owl:Restriction ;
                                                     owl:onProperty cro:InstalledInYear ;
                                                     owl:someValuesFrom xsd:string
                                                   ] ,
                                                   [ rdf:type owl:Restriction ;
                                                     owl:onProperty cro:PCASDescription ;
                                                     owl:someValuesFrom xsd:string
                                                   ] ,
                                                   [ rdf:type owl:Restriction ;
                                                     owl:onProperty cro:PCASName ;
                                                     owl:someValuesFrom xsd:string
                                                   ] ,
                                                   [ rdf:type owl:Restriction ;
                                                     owl:onProperty cro:PCASlocatedIn ;
                                                     owl:someValuesFrom xsd:string
                                                   ] ,
                                                   [ rdf:type owl:Restriction ;
                                                     owl:onProperty cro:electricityDemand ;
                                                     owl:someValuesFrom xsd:string
                                                   ] ,
                                                   [ rdf:type owl:Restriction ;
                                                     owl:onProperty cro:hasPhone ;
                                                     owl:someValuesFrom xsd:string
                                                   ] ,
                                                   [ rdf:type owl:Restriction ;
                                                     owl:onProperty cro:retiredInYear ;
                                                     owl:someValuesFrom xsd:string
                                                   ] ;
                                   rdfs:comment "Process Control Automation System (PCAS) refers to a comprehensive system designed to automate, monitor, and control industrial processes. It typically integrates hardware and software components to ensure precise control, data acquisition, and real-time decision-making in various operational environments." .


###  http://WSP.org/ontology/cro#ProcessingPlant
cro:ProcessingPlant rdf:type owl:Class ;
                    rdfs:subClassOf cro:Facility ,
                                    [ rdf:type owl:Restriction ;
                                      owl:onProperty cro:hasEquipment ;
                                      owl:someValuesFrom cro:Equipment
                                    ] ,
                                    [ rdf:type owl:Restriction ;
                                      owl:onProperty cro:isPartOf ;
                                      owl:someValuesFrom cro:Mine
                                    ] ,
                                    [ rdf:type owl:Restriction ;
                                      owl:onProperty cro:producesTailings ;
                                      owl:someValuesFrom cro:TailingsStorageFacility
                                    ] ,
                                    [ rdf:type owl:Restriction ;
                                      owl:onProperty cro:designCapacity ;
                                      owl:someValuesFrom xsd:decimal
                                    ] ,
                                    [ rdf:type owl:Restriction ;
                                      owl:onProperty cro:oreTypeProcessed ;
                                      owl:someValuesFrom xsd:string
                                    ] .


###  http://WSP.org/ontology/cro#Project
cro:Project rdf:type owl:Class ;
            rdfs:subClassOf [ rdf:type owl:Restriction ;
                              owl:onProperty cro:projectCompletionDate ;
                              owl:someValuesFrom xsd:dateTime
                            ] ,
                            [ rdf:type owl:Restriction ;
                              owl:onProperty cro:projectDescription ;
                              owl:someValuesFrom xsd:string
                            ] ,
                            [ rdf:type owl:Restriction ;
                              owl:onProperty cro:projectName ;
                              owl:someValuesFrom xsd:string
                            ] ,
                            [ rdf:type owl:Restriction ;
                              owl:onProperty cro:supportNetwork ;
                              owl:someValuesFrom xsd:string
                            ] ,
                            [ rdf:type owl:Restriction ;
                              owl:onProperty cro:totalElectricityDemand ;
                              owl:someValuesFrom xsd:decimal
                            ] ,
                            [ rdf:type owl:Restriction ;
                              owl:onProperty cro:workCommencedBoolean ;
                              owl:someValuesFrom xsd:boolean
                            ] ;
            rdfs:comment "A Project represents a structured effort within an operation aimed at achieving specific goals, such as infrastructure upgrades or process improvements." .


###  http://WSP.org/ontology/cro#Recommendation
cro:Recommendation rdf:type owl:Class ;
                   rdfs:subClassOf [ rdf:type owl:Restriction ;
                                     owl:onProperty cro:improvesOperation ;
                                     owl:someValuesFrom cro:Operation
                                   ] ,
                                   [ rdf:type owl:Restriction ;
                                     owl:onProperty cro:recommendationImprovesEquipment ;
                                     owl:someValuesFrom cro:Equipment
                                   ] ,
                                   [ rdf:type owl:Restriction ;
                                     owl:onProperty cro:recommendationImprovesFacility ;
                                     owl:someValuesFrom cro:Facility
                                   ] ,
                                   [ rdf:type owl:Restriction ;
                                     owl:onProperty cro:riskManagementSystemImproved ;
                                     owl:someValuesFrom cro:RiskManagementSystem
                                   ] ,
                                   [ rdf:type owl:Restriction ;
                                     owl:onProperty cro:classification ;
                                     owl:someValuesFrom xsd:string
                                   ] ,
                                   [ rdf:type owl:Restriction ;
                                     owl:onProperty cro:dateCompletedSupersededRejected ;
                                     owl:someValuesFrom xsd:string
                                   ] ,
                                   [ rdf:type owl:Restriction ;
                                     owl:onProperty cro:expenditure ;
                                     owl:someValuesFrom xsd:string
                                   ] ,
                                   [ rdf:type owl:Restriction ;
                                     owl:onProperty cro:likelihoodAfterRecommendation ;
                                     owl:someValuesFrom xsd:string
                                   ] ,
                                   [ rdf:type owl:Restriction ;
                                     owl:onProperty cro:likelihoodNow ;
                                     owl:someValuesFrom xsd:string
                                   ] ,
                                   [ rdf:type owl:Restriction ;
                                     owl:onProperty cro:lossEstimateAfterRecommendationUSDM ;
                                     owl:someValuesFrom xsd:decimal
                                   ] ,
                                   [ rdf:type owl:Restriction ;
                                     owl:onProperty cro:lossEstimateNowUSDM ;
                                     owl:someValuesFrom xsd:decimal
                                   ] ,
                                   [ rdf:type owl:Restriction ;
                                     owl:onProperty cro:positionAccountable ;
                                     owl:someValuesFrom xsd:string
                                   ] ,
                                   [ rdf:type owl:Restriction ;
                                     owl:onProperty cro:recommendationDescription ;
                                     owl:someValuesFrom xsd:string
                                   ] ,
                                   [ rdf:type owl:Restriction ;
                                     owl:onProperty cro:recommendationDetailText ;
                                     owl:someValuesFrom xsd:string
                                   ] ,
                                   [ rdf:type owl:Restriction ;
                                     owl:onProperty cro:recommendationEstimatedCostUSDM ;
                                     owl:someValuesFrom xsd:decimal
                                   ] ,
                                   [ rdf:type owl:Restriction ;
                                     owl:onProperty cro:recommendationPriority ;
                                     owl:someValuesFrom xsd:string
                                   ] ,
                                   [ rdf:type owl:Restriction ;
                                     owl:onProperty cro:recommendationStatus ;
                                     owl:someValuesFrom xsd:string
                                   ] ,
                                   [ rdf:type owl:Restriction ;
                                     owl:onProperty cro:recommendationYear ;
                                     owl:someValuesFrom xsd:string
                                   ] ,
                                   [ rdf:type owl:Restriction ;
                                     owl:onProperty cro:siteResponseOrComments ;
                                     owl:someValuesFrom xsd:string
                                   ] ,
                                   [ rdf:type owl:Restriction ;
                                     owl:onProperty cro:summaryText ;
                                     owl:someValuesFrom xsd:string
                                   ] ;
                   rdfs:comment "Class representing the details of a recommendation." .


###  http://WSP.org/ontology/cro#RecommendationOverview
cro:RecommendationOverview rdf:type owl:Class ;
                           rdfs:subClassOf [ rdf:type owl:Restriction ;
                                             owl:onProperty cro:hasRejectedRecommendations ;
                                             owl:someValuesFrom cro:RejectedRecommendationsSinceLastVisit
                                           ] ,
                                           [ rdf:type owl:Restriction ;
                                             owl:onProperty cro:completeRecommendationNumber ;
                                             owl:someValuesFrom xsd:string
                                           ] ,
                                           [ rdf:type owl:Restriction ;
                                             owl:onProperty cro:highReturnNewRecommendations ;
                                             owl:someValuesFrom xsd:string
                                           ] ,
                                           [ rdf:type owl:Restriction ;
                                             owl:onProperty cro:inProgressRecommendationNumber ;
                                             owl:someValuesFrom xsd:string
                                           ] ,
                                           [ rdf:type owl:Restriction ;
                                             owl:onProperty cro:incrementalImprovementNumber ;
                                             owl:someValuesFrom xsd:string
                                           ] ,
                                           [ rdf:type owl:Restriction ;
                                             owl:onProperty cro:mandarotyNewRecommendations ;
                                             owl:someValuesFrom xsd:string
                                           ] ,
                                           [ rdf:type owl:Restriction ;
                                             owl:onProperty cro:mediumReturnNewRecommendations ;
                                             owl:someValuesFrom xsd:string
                                           ] ,
                                           [ rdf:type owl:Restriction ;
                                             owl:onProperty cro:recommendationDefinition ;
                                             owl:someValuesFrom xsd:string
                                           ] ,
                                           [ rdf:type owl:Restriction ;
                                             owl:onProperty cro:recommendationsCompletedSinceLastReview ;
                                             owl:someValuesFrom xsd:string
                                           ] ,
                                           [ rdf:type owl:Restriction ;
                                             owl:onProperty cro:rejectedRecommendationNumber ;
                                             owl:someValuesFrom xsd:string
                                           ] ,
                                           [ rdf:type owl:Restriction ;
                                             owl:onProperty cro:suspendedRecommendationNumber ;
                                             owl:someValuesFrom xsd:string
                                           ] ,
                                           [ rdf:type owl:Restriction ;
                                             owl:onProperty cro:totalRecommendationNumber ;
                                             owl:someValuesFrom xsd:string
                                           ] ,
                                           [ rdf:type owl:Restriction ;
                                             owl:onProperty cro:underReviewRecommendationNumber ;
                                             owl:someValuesFrom xsd:string
                                           ] ;
                           rdfs:comment "Class representing the overview of recommendations." .


###  http://WSP.org/ontology/cro#ReferenceDocuments
cro:ReferenceDocuments rdf:type owl:Class ;
                       rdfs:subClassOf [ rdf:type owl:Restriction ;
                                         owl:onProperty cro:referenceDocumentDescription ;
                                         owl:someValuesFrom xsd:string
                                       ] ;
                       rdfs:comment "Class representing reference documents for the report." .


###  http://WSP.org/ontology/cro#RejectedRecommendationsSinceLastVisit
cro:RejectedRecommendationsSinceLastVisit rdf:type owl:Class ;
                                          rdfs:subClassOf [ rdf:type owl:Restriction ;
                                                            owl:onProperty cro:rejectedRecommendationDescription ;
                                                            owl:someValuesFrom xsd:string
                                                          ] ;
                                          rdfs:comment "Class representing rejected recommendations since the last visit." .


###  http://WSP.org/ontology/cro#Revision
cro:Revision rdf:type owl:Class ;
             rdfs:subClassOf [ rdf:type owl:Restriction ;
                               owl:onProperty cro:issuedBy ;
                               owl:someValuesFrom cro:Employee
                             ] ,
                             [ rdf:type owl:Restriction ;
                               owl:onProperty cro:checkedBy ;
                               owl:someValuesFrom xsd:string
                             ] ,
                             [ rdf:type owl:Restriction ;
                               owl:onProperty cro:hasDateOfIssue ;
                               owl:someValuesFrom xsd:dateTime
                             ] ,
                             [ rdf:type owl:Restriction ;
                               owl:onProperty cro:hasRevisionDetail ;
                               owl:someValuesFrom xsd:string
                             ] ;
             rdfs:comment "Revision refers to the process of reviewing and updating critical documents, such as CRAs and NATHAN Data, within an operation. Revisions are typically carried out by Employees to ensure accuracy and compliance." .


###  http://WSP.org/ontology/cro#RiskManagementSubElement
cro:RiskManagementSubElement rdf:type owl:Class ;
                             rdfs:subClassOf [ rdf:type owl:Restriction ;
                                               owl:onProperty cro:currentSurveySubElementScore ;
                                               owl:someValuesFrom xsd:int
                                             ] ,
                                             [ rdf:type owl:Restriction ;
                                               owl:onProperty cro:previousSurveySubElementScore ;
                                               owl:someValuesFrom xsd:int
                                             ] ,
                                             [ rdf:type owl:Restriction ;
                                               owl:onProperty cro:riskManagementSubElementInformation ;
                                               owl:someValuesFrom xsd:string
                                             ] .


###  http://WSP.org/ontology/cro#RiskManagementSystem
cro:RiskManagementSystem rdf:type owl:Class ;
                         rdfs:subClassOf [ rdf:type owl:Restriction ;
                                           owl:onProperty cro:hasRiskManagementSubElement ;
                                           owl:someValuesFrom cro:RiskManagementSubElement
                                         ] ,
                                         [ rdf:type owl:Restriction ;
                                           owl:onProperty cro:currentSurveySystemPercentage ;
                                           owl:someValuesFrom xsd:int
                                         ] ,
                                         [ rdf:type owl:Restriction ;
                                           owl:onProperty cro:previousSurveySystemPercentage ;
                                           owl:someValuesFrom xsd:int
                                         ] .


###  http://WSP.org/ontology/cro#SignificantChanges
cro:SignificantChanges rdf:type owl:Class ;
                       rdfs:subClassOf [ rdf:type owl:Restriction ;
                                         owl:onProperty cro:significantChangeDescription ;
                                         owl:someValuesFrom xsd:string
                                       ] ;
                       rdfs:comment "A collection of major updates and modifications identified during the most recent Critical Risk Assessment. A change in the Critical Risk Assesment Report can be: an Organiational Change, a system change, a change to raw materials, production or sales, a change to equipment and facilities, a change to external environment or a change to a specific sritical risk scenario." .


###  http://WSP.org/ontology/cro#SignificantIncident
cro:SignificantIncident rdf:type owl:Class ;
                        rdfs:subClassOf [ rdf:type owl:Restriction ;
                                          owl:onProperty cro:incidentDescription ;
                                          owl:someValuesFrom xsd:string
                                        ] ,
                                        [ rdf:type owl:Restriction ;
                                          owl:onProperty cro:incidentName ;
                                          owl:someValuesFrom xsd:string
                                        ] ,
                                        [ rdf:type owl:Restriction ;
                                          owl:onProperty cro:timeSinceLastIncident ;
                                          owl:someValuesFrom xsd:string
                                        ] ;
                        rdfs:comment "Records of significant incidents that have occurred, including their impact on operations and any resulting changes." .


###  http://WSP.org/ontology/cro#Spillway
cro:Spillway rdf:type owl:Class ;
             rdfs:subClassOf [ rdf:type owl:Restriction ;
                               owl:onProperty cro:connectsTailingsCells ;
                               owl:someValuesFrom cro:TailingsCell
                             ] ,
                             [ rdf:type owl:Restriction ;
                               owl:onProperty cro:spillwayStatus ;
                               owl:someValuesFrom xsd:string
                             ] .


###  http://WSP.org/ontology/cro#Substation
cro:Substation rdf:type owl:Class ;
               rdfs:subClassOf cro:SurveyAndReportDetails ,
                               [ rdf:type owl:Restriction ;
                                 owl:onProperty cro:UpgradeThroughProject ;
                                 owl:someValuesFrom cro:Project
                               ] ,
                               [ rdf:type owl:Restriction ;
                                 owl:onProperty cro:designMaterialSpecification ;
                                 owl:someValuesFrom xsd:string
                               ] ,
                               [ rdf:type owl:Restriction ;
                                 owl:onProperty cro:fireSupressionCondition ;
                                 owl:someValuesFrom xsd:string
                               ] ,
                               [ rdf:type owl:Restriction ;
                                 owl:onProperty cro:substationCondition ;
                                 owl:someValuesFrom xsd:string
                               ] ,
                               [ rdf:type owl:Restriction ;
                                 owl:onProperty cro:substationDescription ;
                                 owl:someValuesFrom xsd:string
                               ] ,
                               [ rdf:type owl:Restriction ;
                                 owl:onProperty cro:substationInstallationDate ;
                                 owl:someValuesFrom xsd:string
                               ] ,
                               [ rdf:type owl:Restriction ;
                                 owl:onProperty cro:substationLocatedIn ;
                                 owl:someValuesFrom xsd:string
                               ] ,
                               [ rdf:type owl:Restriction ;
                                 owl:onProperty cro:substationName ;
                                 owl:someValuesFrom xsd:string
                               ] ;
               rdfs:comment "A facility in the electrical distribution system where voltage is stepped up or down using transformers." ;
               rdfs:label "Substation" .


###  http://WSP.org/ontology/cro#SurveyAndReportDetails
cro:SurveyAndReportDetails rdf:type owl:Class ;
                           rdfs:subClassOf [ rdf:type owl:Restriction ;
                                             owl:onProperty cro:definesRecommendations ;
                                             owl:someValuesFrom cro:RecommendationOverview
                                           ] ,
                                           [ rdf:type owl:Restriction ;
                                             owl:onProperty cro:hasReferenceDocuments ;
                                             owl:someValuesFrom cro:ReferenceDocuments
                                           ] ,
                                           [ rdf:type owl:Restriction ;
                                             owl:onProperty cro:contactDescription ;
                                             owl:someValuesFrom xsd:string
                                           ] ,
                                           [ rdf:type owl:Restriction ;
                                             owl:onProperty cro:generalNotes ;
                                             owl:someValuesFrom xsd:string
                                           ] ;
                           rdfs:comment "Class representing details of the survey and report." .


###  http://WSP.org/ontology/cro#SystemChanges
cro:SystemChanges rdf:type owl:Class ;
                  rdfs:subClassOf cro:SignificantChanges ,
                                  [ rdf:type owl:Restriction ;
                                    owl:onProperty cro:systemChangeDescription ;
                                    owl:someValuesFrom xsd:string
                                  ] ,
                                  [ rdf:type owl:Restriction ;
                                    owl:onProperty cro:systemChangeName ;
                                    owl:someValuesFrom xsd:string
                                  ] ;
                  rdfs:comment "Changes or upgrades to the systems used within the operation, particularly those affecting operational control or data management." .


###  http://WSP.org/ontology/cro#TailingsCell
cro:TailingsCell rdf:type owl:Class ;
                 rdfs:subClassOf [ rdf:type owl:Restriction ;
                                   owl:onProperty cro:capacity ;
                                   owl:someValuesFrom xsd:decimal
                                 ] ,
                                 [ rdf:type owl:Restriction ;
                                   owl:onProperty cro:cellNumber ;
                                   owl:someValuesFrom xsd:int
                                 ] ,
                                 [ rdf:type owl:Restriction ;
                                   owl:onProperty cro:cellStatus ;
                                   owl:someValuesFrom xsd:string
                                 ] ,
                                 [ rdf:type owl:Restriction ;
                                   owl:onProperty cro:dimensions ;
                                   owl:someValuesFrom xsd:decimal
                                 ] ,
                                 [ rdf:type owl:Restriction ;
                                   owl:onProperty cro:expectedFailureDate ;
                                   owl:someValuesFrom xsd:string
                                 ] ,
                                 [ rdf:type owl:Restriction ;
                                   owl:onProperty cro:shape ;
                                   owl:someValuesFrom xsd:string
                                 ] .


###  http://WSP.org/ontology/cro#TailingsStorageFacility
cro:TailingsStorageFacility rdf:type owl:Class ;
                            rdfs:subClassOf cro:Facility ,
                                            [ rdf:type owl:Restriction ;
                                              owl:onProperty cro:hasEmbankment ;
                                              owl:someValuesFrom cro:Embankment
                                            ] ,
                                            [ rdf:type owl:Restriction ;
                                              owl:onProperty cro:hasSpillway ;
                                              owl:someValuesFrom cro:Spillway
                                            ] ,
                                            [ rdf:type owl:Restriction ;
                                              owl:onProperty cro:hasTailingsCell ;
                                              owl:someValuesFrom cro:TailingsCell
                                            ] ,
                                            [ rdf:type owl:Restriction ;
                                              owl:onProperty cro:TSFCapacity ;
                                              owl:someValuesFrom xsd:string
                                            ] ,
                                            [ rdf:type owl:Restriction ;
                                              owl:onProperty cro:TSFConsequenceCategory ;
                                              owl:someValuesFrom xsd:string
                                            ] ,
                                            [ rdf:type owl:Restriction ;
                                              owl:onProperty cro:TSFName ;
                                              owl:someValuesFrom xsd:string
                                            ] ,
                                            [ rdf:type owl:Restriction ;
                                              owl:onProperty cro:TSFStatus ;
                                              owl:someValuesFrom xsd:string
                                            ] .


###  http://WSP.org/ontology/cro#Town
cro:Town rdf:type owl:Class ;
         rdfs:subClassOf [ rdf:type owl:Restriction ;
                           owl:onProperty cro:electricityDemand ;
                           owl:someValuesFrom xsd:string
                         ] ,
                         [ rdf:type owl:Restriction ;
                           owl:onProperty cro:townName ;
                           owl:someValuesFrom xsd:string
                         ] ;
         rdfs:comment "Towns relevant to the operation" .


###  http://WSP.org/ontology/cro#Transformer
cro:Transformer rdf:type owl:Class ;
                rdfs:subClassOf [ rdf:type owl:Restriction ;
                                  owl:onProperty cro:transformerLocatedAtSubstation ;
                                  owl:someValuesFrom cro:Substation
                                ] ,
                                [ rdf:type owl:Restriction ;
                                  owl:onProperty cro:agedConditionBoolean ;
                                  owl:someValuesFrom xsd:boolean
                                ] ,
                                [ rdf:type owl:Restriction ;
                                  owl:onProperty cro:amperage ;
                                  owl:someValuesFrom xsd:string
                                ] ,
                                [ rdf:type owl:Restriction ;
                                  owl:onProperty cro:inputVoltage ;
                                  owl:someValuesFrom xsd:string
                                ] ,
                                [ rdf:type owl:Restriction ;
                                  owl:onProperty cro:installationDate ;
                                  owl:someValuesFrom xsd:string
                                ] ,
                                [ rdf:type owl:Restriction ;
                                  owl:onProperty cro:operationCriticalReliance ;
                                  owl:someValuesFrom xsd:string
                                ] ,
                                [ rdf:type owl:Restriction ;
                                  owl:onProperty cro:outputVoltage ;
                                  owl:someValuesFrom xsd:string
                                ] ;
                rdfs:comment "A device that transfers electrical energy between two or more circuits through electromagnetic induction, used to step up or down voltage levels." .


###  http://WSP.org/ontology/cro#TransmissionLine
cro:TransmissionLine rdf:type owl:Class ;
                     rdfs:subClassOf [ rdf:type owl:Restriction ;
                                       owl:onProperty cro:UpgradeThroughProject ;
                                       owl:someValuesFrom cro:Project
                                     ] ,
                                     [ rdf:type owl:Restriction ;
                                       owl:onProperty cro:connectsFrom ;
                                       owl:someValuesFrom cro:PowerStation
                                     ] ,
                                     [ rdf:type owl:Restriction ;
                                       owl:onProperty cro:connectsTo ;
                                       owl:someValuesFrom cro:Transformer
                                     ] ,
                                     [ rdf:type owl:Restriction ;
                                       owl:onProperty cro:agedConditionBoolean ;
                                       owl:someValuesFrom xsd:boolean
                                     ] ,
                                     [ rdf:type owl:Restriction ;
                                       owl:onProperty cro:installationDate ;
                                       owl:someValuesFrom xsd:string
                                     ] ,
                                     [ rdf:type owl:Restriction ;
                                       owl:onProperty cro:operationCriticalReliance ;
                                       owl:someValuesFrom xsd:string
                                     ] ,
                                     [ rdf:type owl:Restriction ;
                                       owl:onProperty cro:transmissionLineType ;
                                       owl:someValuesFrom xsd:string
                                     ] ,
                                     [ rdf:type owl:Restriction ;
                                       owl:onProperty cro:upgradeYear ;
                                       owl:someValuesFrom xsd:string
                                     ] ,
                                     [ rdf:type owl:Restriction ;
                                       owl:onProperty cro:upgradedBy ;
                                       owl:someValuesFrom xsd:string
                                     ] ,
                                     [ rdf:type owl:Restriction ;
                                       owl:onProperty cro:voltageLevel ;
                                       owl:someValuesFrom xsd:string
                                     ] ;
                     rdfs:comment "High voltage cables used to transmit electricity over long distances." .


###  http://WSP.org/ontology/cro#Turbine
cro:Turbine rdf:type owl:Class ;
            rdfs:subClassOf [ rdf:type owl:Restriction ;
                              owl:onProperty cro:engineCapacity ;
                              owl:someValuesFrom xsd:string
                            ] ,
                            [ rdf:type owl:Restriction ;
                              owl:onProperty cro:engineModel ;
                              owl:someValuesFrom xsd:string
                            ] ,
                            [ rdf:type owl:Restriction ;
                              owl:onProperty cro:runByDieselBoolean ;
                              owl:someValuesFrom xsd:boolean
                            ] ,
                            [ rdf:type owl:Restriction ;
                              owl:onProperty cro:runByGasBoolean ;
                              owl:someValuesFrom xsd:boolean
                            ] ;
            rdfs:comment "A machine that converts energy from a fluid flow into mechanical energy, typically used in electricity generation." .


###  http://WSP.org/ontology/cro#Underground
cro:Underground rdf:type owl:Class ;
                rdfs:subClassOf cro:Mine ,
                                [ rdf:type owl:Restriction ;
                                  owl:onProperty cro:numberOfPanels ;
                                  owl:someValuesFrom xsd:int
                                ] ,
                                [ rdf:type owl:Restriction ;
                                  owl:onProperty cro:numberOfShafts ;
                                  owl:someValuesFrom xsd:int
                                ] ,
                                [ rdf:type owl:Restriction ;
                                  owl:onProperty cro:ventilationAirflow ;
                                  owl:someValuesFrom xsd:string
                                ] .


###  http://WSP.org/ontology/cro#UtilitySuppliersAndConsumables
cro:UtilitySuppliersAndConsumables rdf:type owl:Class ;
                                   rdfs:subClassOf cro:Dependencies ,
                                                   [ rdf:type owl:Restriction ;
                                                     owl:onProperty cro:utilityOrSupplyDescription ;
                                                     owl:someValuesFrom xsd:string
                                                   ] ,
                                                   [ rdf:type owl:Restriction ;
                                                     owl:onProperty cro:utilityOrSupplyName ;
                                                     owl:someValuesFrom xsd:string
                                                   ] ;
                                   rdfs:comment "Class representing utility suppliers and consumables." .


###  Generated by the OWL API (version 4.5.29.2024-05-13T12:11:03Z) https://github.com/owlcs/owlapi
